<?xml version="1.0"?>
<!DOCTYPE rdf:RDF [
    <!ENTITY owl "http://www.w3.org/2002/07/owl#" >
    <!ENTITY obo "http://purl.obolibrary.org/obo/" >
    <!ENTITY dc "http://purl.org/dc/elements/1.1/" >
    <!ENTITY xsd "http://www.w3.org/2001/XMLSchema#" >
    <!ENTITY xml "http://www.w3.org/XML/1998/namespace" >
    <!ENTITY rdfs "http://www.w3.org/2000/01/rdf-schema#" >
    <!ENTITY taxon "http://purl.obolibrary.org/obo/NCBITaxon#" >
    <!ENTITY rdf "http://www.w3.org/1999/02/22-rdf-syntax-ns#" >
    <!ENTITY oboInOwl "http://www.geneontology.org/formats/oboInOwl#" >
    <!ENTITY Lt "&lt;" >
    <!ENTITY Gt "&gt;" >
]>

<rdf:RDF xmlns="http://purl.obolibrary.org/obo/foodon/imports/langual_deprecated_import.owl#"
     xml:base="http://purl.obolibrary.org/obo/foodon/imports/langual_deprecated_import.owl"
     xmlns:rdf="http://www.w3.org/1999/02/22-rdf-syntax-ns#"
     xmlns:owl="http://www.w3.org/2002/07/owl#"
     xmlns:oboInOwl="http://www.geneontology.org/formats/oboInOwl#"
     xmlns:xml="http://www.w3.org/XML/1998/namespace"
     xmlns:xsd="http://www.w3.org/2001/XMLSchema#"
     xmlns:taxon="http://purl.obolibrary.org/obo/NCBITaxon#"
     xmlns:rdfs="http://www.w3.org/2000/01/rdf-schema#"
     xmlns:obo="http://purl.obolibrary.org/obo/"
     xmlns:dc="http://purl.org/dc/elements/1.1/">
    <owl:Ontology rdf:about="http://purl.obolibrary.org/obo/foodon/imports/langual_deprecated_import.owl">
        <dc:contributor xml:lang="en">Damion Dooley</dc:contributor>
    </owl:Ontology>
    

    <!-- For some reason, for annotation <axiom> to work, this exact template has to be in place -->


    <!-- 
    ///////////////////////////////////////////////////////////////////////////////////////
    //
    // Annotation properties
    //
    ///////////////////////////////////////////////////////////////////////////////////////
     -->


    <!-- http://purl.obolibrary.org/obo/IAO_0000114 -->

    <owl:AnnotationProperty rdf:about="http://purl.obolibrary.org/obo/IAO_0000114"/>
    


    <!-- http://purl.obolibrary.org/obo/IAO_0000115 -->

    <owl:AnnotationProperty rdf:about="http://purl.obolibrary.org/obo/IAO_0000115"/>
    


    <!-- http://purl.obolibrary.org/obo/IAO_0000412 -->

    <owl:AnnotationProperty rdf:about="http://purl.obolibrary.org/obo/IAO_0000412"/>
    


    <!-- http://www.geneontology.org/formats/oboInOwl#hasBroadSynonym -->

    <owl:AnnotationProperty rdf:about="http://www.geneontology.org/formats/oboInOwl#hasBroadSynonym"/>
    


    <!-- http://www.geneontology.org/formats/oboInOwl#hasDbXref -->

    <owl:AnnotationProperty rdf:about="http://www.geneontology.org/formats/oboInOwl#hasDbXref"/>
    


    <!-- http://www.geneontology.org/formats/oboInOwl#hasNarrowSynonym -->

    <owl:AnnotationProperty rdf:about="http://www.geneontology.org/formats/oboInOwl#hasNarrowSynonym"/>
    


    <!-- http://www.geneontology.org/formats/oboInOwl#hasSynonym -->

    <owl:AnnotationProperty rdf:about="http://www.geneontology.org/formats/oboInOwl#hasSynonym"/>
    


    <!-- 
    ///////////////////////////////////////////////////////////////////////////////////////
    //
    // Object Properties
    //
    ///////////////////////////////////////////////////////////////////////////////////////
     -->

    


    <!-- http://purl.obolibrary.org/obo/RO_0000087 -->

    <owl:ObjectProperty rdf:about="http://purl.obolibrary.org/obo/RO_0000087"/>
    


    <!-- 
    ///////////////////////////////////////////////////////////////////////////////////////
    //
    // Classes
    //
    ///////////////////////////////////////////////////////////////////////////////////////
     -->

    


<owl:Class rdf:about="&obo;FOODON_03400000">
	<rdfs:label xml:lang="en">langual thesaurus root</rdfs:label>
	<rdfs:subClassOf rdf:resource="http://www.geneontology.org/formats/oboInOwl#ObsoleteClass"/>
	<obo:IAO_0000412>http://langual.org</obo:IAO_0000412>
	<obo:IAO_0000115 xml:lang="en">2014</obo:IAO_0000115>
	<owl:deprecated rdf:datatype="&xsd;boolean">true</owl:deprecated>
	<obo:IAO_0000114 rdf:resource="&obo;IAO_0000122"/>
	<rdfs:comment xml:lang="en">LanguaL curation note: This term is for CLASSIFICATION ONLY; DO NOT USE term in indexing. Use a more precise narrower term.</rdfs:comment>
	<oboInOwl:hasDbXref>LANGUAL:00000</oboInOwl:hasDbXref>
</owl:Class>

<owl:Class rdf:about="&obo;FOODON_03410001">
	<rdfs:label xml:lang="en">food source not known</rdfs:label>
	<rdfs:subClassOf rdf:resource="http://www.geneontology.org/formats/oboInOwl#ObsoleteClass"/>
	<obo:IAO_0000412>http://langual.org</obo:IAO_0000412>
	<owl:deprecated rdf:datatype="&xsd;boolean">true</owl:deprecated>
	<obo:IAO_0000114 rdf:resource="&obo;IAO_0000122"/>
	<rdfs:comment xml:lang="en">LanguaL curation note: Used only if so little is known about the food source that not even *ANIMAL USED AS FOOD SOURCE*, *PLANT USED AS FOOD SOURCE*, *ALGAE OR FUNGUS AS FOOD SOURCE* or *CHEMICAL FOOD SOURCE* can be assigned.</rdfs:comment>
	<oboInOwl:hasDbXref>LANGUAL:B0001</oboInOwl:hasDbXref>
</owl:Class>

<owl:Class rdf:about="&obo;FOODON_03411000">
	<rdfs:label xml:lang="en">cattle and swine and calf</rdfs:label>
	<rdfs:subClassOf rdf:resource="http://www.geneontology.org/formats/oboInOwl#ObsoleteClass"/>
	<obo:IAO_0000412>http://langual.org</obo:IAO_0000412>
	<owl:deprecated rdf:datatype="&xsd;boolean">true</owl:deprecated>
	<obo:IAO_0000114 rdf:resource="&obo;IAO_0000122"/>
	<oboInOwl:hasSynonym xml:lang="en">beef and pork and veal</oboInOwl:hasSynonym>
	<oboInOwl:hasSynonym xml:lang="en">calf and cattle and swine</oboInOwl:hasSynonym>
	<oboInOwl:hasSynonym xml:lang="en">calf and swine and cattle</oboInOwl:hasSynonym>
	<oboInOwl:hasSynonym xml:lang="en">swine and cattle and calf</oboInOwl:hasSynonym>
	<oboInOwl:hasDbXref>LANGUAL:B1000</oboInOwl:hasDbXref>
</owl:Class>

<owl:Class rdf:about="&obo;FOODON_03411028">
	<rdfs:label xml:lang="en">grapefruit and orange</rdfs:label>
	<rdfs:subClassOf rdf:resource="http://www.geneontology.org/formats/oboInOwl#ObsoleteClass"/>
	<obo:IAO_0000412>http://langual.org</obo:IAO_0000412>
	<owl:deprecated rdf:datatype="&xsd;boolean">true</owl:deprecated>
	<obo:IAO_0000114 rdf:resource="&obo;IAO_0000122"/>
	<oboInOwl:hasSynonym xml:lang="en">orange and grapefruit</oboInOwl:hasSynonym>
	<oboInOwl:hasDbXref>LANGUAL:B1028</oboInOwl:hasDbXref>
</owl:Class>

<owl:Class rdf:about="&obo;FOODON_03411032">
	<rdfs:label xml:lang="en">sole, species not known</rdfs:label>
	<rdfs:subClassOf rdf:resource="http://www.geneontology.org/formats/oboInOwl#ObsoleteClass"/>
	<obo:IAO_0000412>http://langual.org</obo:IAO_0000412>
	<owl:deprecated rdf:datatype="&xsd;boolean">true</owl:deprecated>
	<obo:IAO_0000114 rdf:resource="&obo;IAO_0000122"/>
	<oboInOwl:hasDbXref>LANGUAL:B1032</oboInOwl:hasDbXref>
</owl:Class>

<owl:Class rdf:about="&obo;FOODON_03411105">
	<rdfs:label xml:lang="en">cattle and swine</rdfs:label>
	<rdfs:subClassOf rdf:resource="http://www.geneontology.org/formats/oboInOwl#ObsoleteClass"/>
	<obo:IAO_0000412>http://langual.org</obo:IAO_0000412>
	<owl:deprecated rdf:datatype="&xsd;boolean">true</owl:deprecated>
	<obo:IAO_0000114 rdf:resource="&obo;IAO_0000122"/>
	<oboInOwl:hasSynonym xml:lang="en">beef and pork</oboInOwl:hasSynonym>
	<oboInOwl:hasSynonym xml:lang="en">swine and cattle</oboInOwl:hasSynonym>
	<oboInOwl:hasDbXref>LANGUAL:B1105</oboInOwl:hasDbXref>
</owl:Class>

<owl:Class rdf:about="&obo;FOODON_03411207">
	<rdfs:label xml:lang="en">prune</rdfs:label>
	<rdfs:subClassOf rdf:resource="http://www.geneontology.org/formats/oboInOwl#ObsoleteClass"/>
	<obo:IAO_0000412>http://langual.org</obo:IAO_0000412>
	<owl:deprecated rdf:datatype="&xsd;boolean">true</owl:deprecated>
	<obo:IAO_0000114 rdf:resource="&obo;IAO_0000122"/>
	<rdfs:comment xml:lang="en">LanguaL curation note: This term is only kept for backward compatibility. DO NOT USE for new indexing.</rdfs:comment>
	<oboInOwl:hasDbXref>LANGUAL:B1207</oboInOwl:hasDbXref>
</owl:Class>

<owl:Class rdf:about="&obo;FOODON_03411246">
	<rdfs:label xml:lang="en">pineapple and grapefruit</rdfs:label>
	<rdfs:subClassOf rdf:resource="http://www.geneontology.org/formats/oboInOwl#ObsoleteClass"/>
	<obo:IAO_0000412>http://langual.org</obo:IAO_0000412>
	<owl:deprecated rdf:datatype="&xsd;boolean">true</owl:deprecated>
	<obo:IAO_0000114 rdf:resource="&obo;IAO_0000122"/>
	<oboInOwl:hasSynonym xml:lang="en">grapefruit and pineapple</oboInOwl:hasSynonym>
	<oboInOwl:hasDbXref>LANGUAL:B1246</oboInOwl:hasDbXref>
</owl:Class>

<owl:Class rdf:about="&obo;FOODON_03411321">
	<rdfs:label xml:lang="en">mace</rdfs:label>
	<rdfs:subClassOf rdf:resource="http://www.geneontology.org/formats/oboInOwl#ObsoleteClass"/>
	<obo:IAO_0000412>http://langual.org</obo:IAO_0000412>
	<owl:deprecated rdf:datatype="&xsd;boolean">true</owl:deprecated>
	<obo:IAO_0000114 rdf:resource="&obo;IAO_0000122"/>
	<rdfs:comment xml:lang="en">LanguaL curation note: This term is only kept for backward compatibility. DO NOT USE for new indexing.</rdfs:comment>
	<oboInOwl:hasDbXref>LANGUAL:B1321</oboInOwl:hasDbXref>
</owl:Class>

<owl:Class rdf:about="&obo;FOODON_03411424">
	<rdfs:label xml:lang="en">blue pike</rdfs:label>
	<rdfs:subClassOf rdf:resource="http://www.geneontology.org/formats/oboInOwl#ObsoleteClass"/>
	<obo:IAO_0000412>http://langual.org</obo:IAO_0000412>
	<obo:IAO_0000115 xml:lang="en">Synonym of *WALLEYE PIKE [B1398]*.</obo:IAO_0000115>
	<owl:deprecated rdf:datatype="&xsd;boolean">true</owl:deprecated>
	<obo:IAO_0000114 rdf:resource="&obo;IAO_0000122"/>
	<rdfs:comment xml:lang="en">LanguaL curation note: This term is only kept for backward compatibility. DO NOT USE for new indexing.</rdfs:comment>
	<oboInOwl:hasDbXref>LANGUAL:B1424</oboInOwl:hasDbXref>
</owl:Class>

<owl:Class rdf:about="&obo;FOODON_03411525">
	<rdfs:label xml:lang="en">peanut with other nut or seed</rdfs:label>
	<rdfs:subClassOf rdf:resource="http://www.geneontology.org/formats/oboInOwl#ObsoleteClass"/>
	<obo:IAO_0000412>http://langual.org</obo:IAO_0000412>
	<owl:deprecated rdf:datatype="&xsd;boolean">true</owl:deprecated>
	<obo:IAO_0000114 rdf:resource="&obo;IAO_0000122"/>
	<oboInOwl:hasDbXref>LANGUAL:B1525</oboInOwl:hasDbXref>
</owl:Class>

<owl:Class rdf:about="&obo;FOODON_03411526">
	<rdfs:label xml:lang="en">weakfish</rdfs:label>
	<rdfs:subClassOf rdf:resource="http://www.geneontology.org/formats/oboInOwl#ObsoleteClass"/>
	<obo:IAO_0000412>http://langual.org</obo:IAO_0000412>
	<owl:deprecated rdf:datatype="&xsd;boolean">true</owl:deprecated>
	<obo:IAO_0000114 rdf:resource="&obo;IAO_0000122"/>
	<rdfs:comment xml:lang="en">LanguaL curation note: This term is only kept for backward compatibility. DO NOT USE for new indexing.</rdfs:comment>
	<obo:IAO_0100001 rdf:resource="&obo;FOODON_03412375"/>
	<oboInOwl:hasDbXref>LANGUAL:B1526</oboInOwl:hasDbXref>
</owl:Class>

<owl:Class rdf:about="&obo;FOODON_03411605">
	<rdfs:label xml:lang="en">pea and onion</rdfs:label>
	<rdfs:subClassOf rdf:resource="http://www.geneontology.org/formats/oboInOwl#ObsoleteClass"/>
	<obo:IAO_0000412>http://langual.org</obo:IAO_0000412>
	<owl:deprecated rdf:datatype="&xsd;boolean">true</owl:deprecated>
	<obo:IAO_0000114 rdf:resource="&obo;IAO_0000122"/>
	<oboInOwl:hasSynonym xml:lang="en">onion and pea</oboInOwl:hasSynonym>
	<oboInOwl:hasDbXref>LANGUAL:B1605</oboInOwl:hasDbXref>
</owl:Class>

<owl:Class rdf:about="&obo;FOODON_03411613">
	<rdfs:label xml:lang="en">pea and carrot</rdfs:label>
	<rdfs:subClassOf rdf:resource="http://www.geneontology.org/formats/oboInOwl#ObsoleteClass"/>
	<obo:IAO_0000412>http://langual.org</obo:IAO_0000412>
	<owl:deprecated rdf:datatype="&xsd;boolean">true</owl:deprecated>
	<obo:IAO_0000114 rdf:resource="&obo;IAO_0000122"/>
	<oboInOwl:hasSynonym xml:lang="en">carrot and pea</oboInOwl:hasSynonym>
	<oboInOwl:hasDbXref>LANGUAL:B1613</oboInOwl:hasDbXref>
</owl:Class>

<owl:Class rdf:about="&obo;FOODON_03411619">
	<rdfs:label xml:lang="en">reindeer</rdfs:label>
	<rdfs:subClassOf rdf:resource="http://www.geneontology.org/formats/oboInOwl#ObsoleteClass"/>
	<obo:IAO_0000412>http://langual.org</obo:IAO_0000412>
	<obo:IAO_0000115 xml:lang="en">Duplicate entry.</obo:IAO_0000115>
	<owl:deprecated rdf:datatype="&xsd;boolean">true</owl:deprecated>
	<obo:IAO_0000114 rdf:resource="&obo;IAO_0000122"/>
	<rdfs:comment xml:lang="en">LanguaL curation note: This term is only kept for backward compatibility. DO NOT USE for new indexing.</rdfs:comment>
	<oboInOwl:hasDbXref>LANGUAL:B1619</oboInOwl:hasDbXref>
</owl:Class>

<owl:Class rdf:about="&obo;FOODON_03411631">
	<rdfs:label xml:lang="en">pineapple and orange</rdfs:label>
	<rdfs:subClassOf rdf:resource="http://www.geneontology.org/formats/oboInOwl#ObsoleteClass"/>
	<obo:IAO_0000412>http://langual.org</obo:IAO_0000412>
	<owl:deprecated rdf:datatype="&xsd;boolean">true</owl:deprecated>
	<obo:IAO_0000114 rdf:resource="&obo;IAO_0000122"/>
	<oboInOwl:hasSynonym xml:lang="en">orange and pineapple</oboInOwl:hasSynonym>
	<oboInOwl:hasDbXref>LANGUAL:B1631</oboInOwl:hasDbXref>
</owl:Class>

<owl:Class rdf:about="&obo;FOODON_03411680">
	<rdfs:label xml:lang="en">sugar cane and field corn</rdfs:label>
	<rdfs:subClassOf rdf:resource="http://www.geneontology.org/formats/oboInOwl#ObsoleteClass"/>
	<obo:IAO_0000412>http://langual.org</obo:IAO_0000412>
	<owl:deprecated rdf:datatype="&xsd;boolean">true</owl:deprecated>
	<obo:IAO_0000114 rdf:resource="&obo;IAO_0000122"/>
	<oboInOwl:hasSynonym xml:lang="en">field corn and sugar cane</oboInOwl:hasSynonym>
	<oboInOwl:hasDbXref>LANGUAL:B1680</oboInOwl:hasDbXref>
</owl:Class>

<owl:Class rdf:about="&obo;FOODON_03411709">
	<rdfs:label xml:lang="en">orange and apricot</rdfs:label>
	<rdfs:subClassOf rdf:resource="http://www.geneontology.org/formats/oboInOwl#ObsoleteClass"/>
	<obo:IAO_0000412>http://langual.org</obo:IAO_0000412>
	<owl:deprecated rdf:datatype="&xsd;boolean">true</owl:deprecated>
	<obo:IAO_0000114 rdf:resource="&obo;IAO_0000122"/>
	<oboInOwl:hasSynonym xml:lang="en">apricot and orange</oboInOwl:hasSynonym>
	<oboInOwl:hasDbXref>LANGUAL:B1709</oboInOwl:hasDbXref>
</owl:Class>

<owl:Class rdf:about="&obo;FOODON_03411779">
	<rdfs:label xml:lang="en">california yellowtail</rdfs:label>
	<rdfs:subClassOf rdf:resource="http://www.geneontology.org/formats/oboInOwl#ObsoleteClass"/>
	<obo:IAO_0000412>http://langual.org</obo:IAO_0000412>
	<obo:IAO_0000115 xml:lang="en">Duplicate entry of *YELLOWTAIL [B1779]*.
&lt;SCISYN&gt;Seriola dorsalis (Gill, 1863)</obo:IAO_0000115>
	<owl:deprecated rdf:datatype="&xsd;boolean">true</owl:deprecated>
	<obo:IAO_0000114 rdf:resource="&obo;IAO_0000122"/>
	<rdfs:comment xml:lang="en">LanguaL curation note: This term is only kept for backward compatibility. DO NOT USE for new indexing.</rdfs:comment>
	<obo:IAO_0100001 rdf:resource="&obo;FOODON_03411779"/>
	<oboInOwl:hasDbXref>LANGUAL:B1779</oboInOwl:hasDbXref>
</owl:Class>

<owl:Class rdf:about="&obo;FOODON_03411847">
	<rdfs:label xml:lang="en">pacific sardine</rdfs:label>
	<rdfs:subClassOf rdf:resource="http://www.geneontology.org/formats/oboInOwl#ObsoleteClass"/>
	<obo:IAO_0000412>http://langual.org</obo:IAO_0000412>
	<obo:IAO_0000115 xml:lang="en">Synonym of *CHILEAN PILCHARD [B1847]*</obo:IAO_0000115>
	<owl:deprecated rdf:datatype="&xsd;boolean">true</owl:deprecated>
	<obo:IAO_0000114 rdf:resource="&obo;IAO_0000122"/>
	<rdfs:comment xml:lang="en">LanguaL curation note: This term is only kept for backward compatibility. DO NOT USE for new indexing.</rdfs:comment>
	<oboInOwl:hasDbXref>LANGUAL:B1847</oboInOwl:hasDbXref>
</owl:Class>

<owl:Class rdf:about="&obo;FOODON_03411953">
	<rdfs:label xml:lang="en">ocean quahog</rdfs:label>
	<rdfs:subClassOf rdf:resource="http://www.geneontology.org/formats/oboInOwl#ObsoleteClass"/>
	<obo:IAO_0000412>http://langual.org</obo:IAO_0000412>
	<obo:IAO_0000115 xml:lang="en">Descriptor inactivated due to duplication.</obo:IAO_0000115>
	<owl:deprecated rdf:datatype="&xsd;boolean">true</owl:deprecated>
	<obo:IAO_0000114 rdf:resource="&obo;IAO_0000122"/>
	<rdfs:comment xml:lang="en">LanguaL curation note: This term is only kept for backward compatibility. DO NOT USE for new indexing.</rdfs:comment>
	<oboInOwl:hasDbXref>LANGUAL:B1953</oboInOwl:hasDbXref>
</owl:Class>

<owl:Class rdf:about="&obo;FOODON_03412101">
	<rdfs:label xml:lang="en">sheep and goat</rdfs:label>
	<rdfs:subClassOf rdf:resource="http://www.geneontology.org/formats/oboInOwl#ObsoleteClass"/>
	<obo:IAO_0000412>http://langual.org</obo:IAO_0000412>
	<owl:deprecated rdf:datatype="&xsd;boolean">true</owl:deprecated>
	<obo:IAO_0000114 rdf:resource="&obo;IAO_0000122"/>
	<oboInOwl:hasSynonym xml:lang="en">goat and sheep</oboInOwl:hasSynonym>
	<oboInOwl:hasDbXref>LANGUAL:B2101</oboInOwl:hasDbXref>
</owl:Class>

<owl:Class rdf:about="&obo;FOODON_03412201">
	<rdfs:label xml:lang="en">panulirus rissore</rdfs:label>
	<rdfs:subClassOf rdf:resource="http://www.geneontology.org/formats/oboInOwl#ObsoleteClass"/>
	<obo:IAO_0000412>http://langual.org</obo:IAO_0000412>
	<obo:IAO_0000115 xml:lang="en">Descriptor inactivated.</obo:IAO_0000115>
	<owl:deprecated rdf:datatype="&xsd;boolean">true</owl:deprecated>
	<obo:IAO_0000114 rdf:resource="&obo;IAO_0000122"/>
	<rdfs:comment xml:lang="en">LanguaL curation note: This term is only kept for backward compatibility. DO NOT USE for new indexing.</rdfs:comment>
	<oboInOwl:hasDbXref>LANGUAL:B2201</oboInOwl:hasDbXref>
</owl:Class>

<owl:Class rdf:about="&obo;FOODON_03412242">
	<rdfs:label xml:lang="en">swine and calf</rdfs:label>
	<rdfs:subClassOf rdf:resource="http://www.geneontology.org/formats/oboInOwl#ObsoleteClass"/>
	<obo:IAO_0000412>http://langual.org</obo:IAO_0000412>
	<owl:deprecated rdf:datatype="&xsd;boolean">true</owl:deprecated>
	<obo:IAO_0000114 rdf:resource="&obo;IAO_0000122"/>
	<oboInOwl:hasSynonym xml:lang="en">calf and swine</oboInOwl:hasSynonym>
	<oboInOwl:hasDbXref>LANGUAL:B2242</oboInOwl:hasDbXref>
</owl:Class>

<owl:Class rdf:about="&obo;FOODON_03412243">
	<rdfs:label xml:lang="en">cattle and swine and sheep</rdfs:label>
	<rdfs:subClassOf rdf:resource="http://www.geneontology.org/formats/oboInOwl#ObsoleteClass"/>
	<obo:IAO_0000412>http://langual.org</obo:IAO_0000412>
	<owl:deprecated rdf:datatype="&xsd;boolean">true</owl:deprecated>
	<obo:IAO_0000114 rdf:resource="&obo;IAO_0000122"/>
	<oboInOwl:hasSynonym xml:lang="en">sheep and cattle and swine</oboInOwl:hasSynonym>
	<oboInOwl:hasSynonym xml:lang="en">swine and cattle and sheep</oboInOwl:hasSynonym>
	<oboInOwl:hasDbXref>LANGUAL:B2243</oboInOwl:hasDbXref>
</owl:Class>

<owl:Class rdf:about="&obo;FOODON_03412244">
	<rdfs:label xml:lang="en">cattle and sheep</rdfs:label>
	<rdfs:subClassOf rdf:resource="http://www.geneontology.org/formats/oboInOwl#ObsoleteClass"/>
	<obo:IAO_0000412>http://langual.org</obo:IAO_0000412>
	<owl:deprecated rdf:datatype="&xsd;boolean">true</owl:deprecated>
	<obo:IAO_0000114 rdf:resource="&obo;IAO_0000122"/>
	<oboInOwl:hasSynonym xml:lang="en">cow and sheep</oboInOwl:hasSynonym>
	<oboInOwl:hasSynonym xml:lang="en">sheep and cattle</oboInOwl:hasSynonym>
	<oboInOwl:hasSynonym xml:lang="en">sheep and cow</oboInOwl:hasSynonym>
	<oboInOwl:hasDbXref>LANGUAL:B2244</oboInOwl:hasDbXref>
</owl:Class>

<owl:Class rdf:about="&obo;FOODON_03412245">
	<rdfs:label xml:lang="en">cattle and goat</rdfs:label>
	<rdfs:subClassOf rdf:resource="http://www.geneontology.org/formats/oboInOwl#ObsoleteClass"/>
	<obo:IAO_0000412>http://langual.org</obo:IAO_0000412>
	<owl:deprecated rdf:datatype="&xsd;boolean">true</owl:deprecated>
	<obo:IAO_0000114 rdf:resource="&obo;IAO_0000122"/>
	<oboInOwl:hasSynonym xml:lang="en">cow and goat</oboInOwl:hasSynonym>
	<oboInOwl:hasSynonym xml:lang="en">goat and cattle</oboInOwl:hasSynonym>
	<oboInOwl:hasSynonym xml:lang="en">goat and cow</oboInOwl:hasSynonym>
	<oboInOwl:hasDbXref>LANGUAL:B2245</oboInOwl:hasDbXref>
</owl:Class>

<owl:Class rdf:about="&obo;FOODON_03412247">
	<rdfs:label xml:lang="en">cattle and sheep and goat</rdfs:label>
	<rdfs:subClassOf rdf:resource="http://www.geneontology.org/formats/oboInOwl#ObsoleteClass"/>
	<obo:IAO_0000412>http://langual.org</obo:IAO_0000412>
	<owl:deprecated rdf:datatype="&xsd;boolean">true</owl:deprecated>
	<obo:IAO_0000114 rdf:resource="&obo;IAO_0000122"/>
	<oboInOwl:hasSynonym xml:lang="en">cow and sheep and goat</oboInOwl:hasSynonym>
	<oboInOwl:hasSynonym xml:lang="en">goat and cattle and sheep</oboInOwl:hasSynonym>
	<oboInOwl:hasSynonym xml:lang="en">goat and sheep and cow</oboInOwl:hasSynonym>
	<oboInOwl:hasSynonym xml:lang="en">sheep and cattle and goat</oboInOwl:hasSynonym>
	<oboInOwl:hasSynonym xml:lang="en">sheep and goat and cow</oboInOwl:hasSynonym>
	<oboInOwl:hasDbXref>LANGUAL:B2247</oboInOwl:hasDbXref>
</owl:Class>

<owl:Class rdf:about="&obo;FOODON_03412282">
	<rdfs:label xml:lang="en">school shark</rdfs:label>
	<rdfs:subClassOf rdf:resource="http://www.geneontology.org/formats/oboInOwl#ObsoleteClass"/>
	<obo:IAO_0000412>http://langual.org</obo:IAO_0000412>
	<obo:IAO_0000115 xml:lang="en">School shark is a synonym of TOPE SHARK [B2525], which should be used instead.</obo:IAO_0000115>
	<owl:deprecated rdf:datatype="&xsd;boolean">true</owl:deprecated>
	<obo:IAO_0000114 rdf:resource="&obo;IAO_0000122"/>
	<rdfs:comment xml:lang="en">LanguaL curation note: This term is only kept for backward compatibility. DO NOT USE for new indexing.</rdfs:comment>
	<oboInOwl:hasDbXref>LANGUAL:B2282</oboInOwl:hasDbXref>
</owl:Class>

<owl:Class rdf:about="&obo;FOODON_03412379">
	<rdfs:label xml:lang="en">carmine cusk-eel</rdfs:label>
	<rdfs:subClassOf rdf:resource="http://www.geneontology.org/formats/oboInOwl#ObsoleteClass"/>
	<obo:IAO_0000412>http://langual.org</obo:IAO_0000412>
	<owl:deprecated rdf:datatype="&xsd;boolean">true</owl:deprecated>
	<obo:IAO_0000114 rdf:resource="&obo;IAO_0000122"/>
	<rdfs:comment xml:lang="en">LanguaL curation note: This term is only kept for backward compatibility. DO NOT USE for new indexing.</rdfs:comment>
	<oboInOwl:hasDbXref>LANGUAL:B2379</oboInOwl:hasDbXref>
</owl:Class>

<owl:Class rdf:about="&obo;FOODON_03412381">
	<rdfs:label xml:lang="en">lutjanus silla</rdfs:label>
	<rdfs:subClassOf rdf:resource="http://www.geneontology.org/formats/oboInOwl#ObsoleteClass"/>
	<obo:IAO_0000412>http://langual.org</obo:IAO_0000412>
	<obo:IAO_0000115 xml:lang="en">Species unknown.</obo:IAO_0000115>
	<owl:deprecated rdf:datatype="&xsd;boolean">true</owl:deprecated>
	<obo:IAO_0000114 rdf:resource="&obo;IAO_0000122"/>
	<rdfs:comment xml:lang="en">LanguaL curation note: This term is only kept for backward compatibility. DO NOT USE for new indexing.</rdfs:comment>
	<oboInOwl:hasDbXref>LANGUAL:B2381</oboInOwl:hasDbXref>
</owl:Class>

<owl:Class rdf:about="&obo;FOODON_03412387">
	<rdfs:label xml:lang="en">zander</rdfs:label>
	<rdfs:subClassOf rdf:resource="http://www.geneontology.org/formats/oboInOwl#ObsoleteClass"/>
	<obo:IAO_0000412>http://langual.org</obo:IAO_0000412>
	<obo:IAO_0000115 xml:lang="en">Synonym of *PIKE PERCH [B1399]*</obo:IAO_0000115>
	<owl:deprecated rdf:datatype="&xsd;boolean">true</owl:deprecated>
	<obo:IAO_0000114 rdf:resource="&obo;IAO_0000122"/>
	<rdfs:comment xml:lang="en">LanguaL curation note: This term is only kept for backward compatibility. DO NOT USE for new indexing.</rdfs:comment>
	<oboInOwl:hasDbXref>LANGUAL:B2387</oboInOwl:hasDbXref>
</owl:Class>

<owl:Class rdf:about="&obo;FOODON_03412396">
	<rdfs:label xml:lang="en">cattle and lamb</rdfs:label>
	<rdfs:subClassOf rdf:resource="http://www.geneontology.org/formats/oboInOwl#ObsoleteClass"/>
	<obo:IAO_0000412>http://langual.org</obo:IAO_0000412>
	<owl:deprecated rdf:datatype="&xsd;boolean">true</owl:deprecated>
	<obo:IAO_0000114 rdf:resource="&obo;IAO_0000122"/>
	<oboInOwl:hasDbXref>LANGUAL:B2396</oboInOwl:hasDbXref>
</owl:Class>

<owl:Class rdf:about="&obo;FOODON_03412466">
	<rdfs:label xml:lang="en">snow pea</rdfs:label>
	<rdfs:subClassOf rdf:resource="http://www.geneontology.org/formats/oboInOwl#ObsoleteClass"/>
	<obo:IAO_0000412>http://langual.org</obo:IAO_0000412>
	<owl:deprecated rdf:datatype="&xsd;boolean">true</owl:deprecated>
	<obo:IAO_0000114 rdf:resource="&obo;IAO_0000122"/>
	<rdfs:comment xml:lang="en">LanguaL curation note: This term is only kept for backward compatibility. DO NOT USE for new indexing.</rdfs:comment>
	<oboInOwl:hasDbXref>LANGUAL:B2466</oboInOwl:hasDbXref>
</owl:Class>

<owl:Class rdf:about="&obo;FOODON_03412467">
	<rdfs:label xml:lang="en">sugar pea, edible pod</rdfs:label>
	<rdfs:subClassOf rdf:resource="http://www.geneontology.org/formats/oboInOwl#ObsoleteClass"/>
	<obo:IAO_0000412>http://langual.org</obo:IAO_0000412>
	<owl:deprecated rdf:datatype="&xsd;boolean">true</owl:deprecated>
	<obo:IAO_0000114 rdf:resource="&obo;IAO_0000122"/>
	<rdfs:comment xml:lang="en">LanguaL curation note: This term is only kept for backward compatibility. DO NOT USE for new indexing.</rdfs:comment>
	<oboInOwl:hasDbXref>LANGUAL:B2467</oboInOwl:hasDbXref>
</owl:Class>

<owl:Class rdf:about="&obo;FOODON_03412664">
	<rdfs:label xml:lang="en">corvina</rdfs:label>
	<rdfs:subClassOf rdf:resource="http://www.geneontology.org/formats/oboInOwl#ObsoleteClass"/>
	<obo:IAO_0000412>http://langual.org</obo:IAO_0000412>
	<owl:deprecated rdf:datatype="&xsd;boolean">true</owl:deprecated>
	<obo:IAO_0000114 rdf:resource="&obo;IAO_0000122"/>
	<rdfs:comment xml:lang="en">LanguaL curation note: This term is only kept for backward compatibility. DO NOT USE for new indexing.</rdfs:comment>
	<obo:IAO_0100001 rdf:resource="&obo;FOODON_03411814"/>
	<oboInOwl:hasDbXref>LANGUAL:B2664</oboInOwl:hasDbXref>
</owl:Class>

<owl:Class rdf:about="&obo;FOODON_03412700">
	<rdfs:label xml:lang="en">eel, freshwater</rdfs:label>
	<rdfs:subClassOf rdf:resource="http://www.geneontology.org/formats/oboInOwl#ObsoleteClass"/>
	<obo:IAO_0000412>http://langual.org</obo:IAO_0000412>
	<obo:IAO_0000115 xml:lang="en">FDA market name for Amercan eel, Anguilla rostrata (Lesueur, 1817).</obo:IAO_0000115>
	<owl:deprecated rdf:datatype="&xsd;boolean">true</owl:deprecated>
	<obo:IAO_0000114 rdf:resource="&obo;IAO_0000122"/>
	<rdfs:comment xml:lang="en">LanguaL curation note: This term is only kept for backward compatibility. DO NOT USE for new indexing.</rdfs:comment>
	<oboInOwl:hasDbXref>LANGUAL:B2700</oboInOwl:hasDbXref>
</owl:Class>

<owl:Class rdf:about="&obo;FOODON_03412826">
	<rdfs:label xml:lang="en">belwisia</rdfs:label>
	<rdfs:subClassOf rdf:resource="http://www.geneontology.org/formats/oboInOwl#ObsoleteClass"/>
	<obo:IAO_0000412>http://langual.org</obo:IAO_0000412>
	<obo:IAO_0000115 xml:lang="en">Species unknown.</obo:IAO_0000115>
	<owl:deprecated rdf:datatype="&xsd;boolean">true</owl:deprecated>
	<obo:IAO_0000114 rdf:resource="&obo;IAO_0000122"/>
	<rdfs:comment xml:lang="en">LanguaL curation note: This term is only kept for backward compatibility. DO NOT USE for new indexing.</rdfs:comment>
	<oboInOwl:hasDbXref>LANGUAL:B2826</oboInOwl:hasDbXref>
</owl:Class>

<owl:Class rdf:about="&obo;FOODON_03413066">
	<rdfs:label xml:lang="en">citric acid</rdfs:label>
	<rdfs:subClassOf rdf:resource="http://www.geneontology.org/formats/oboInOwl#ObsoleteClass"/>
	<obo:IAO_0000412>http://langual.org</obo:IAO_0000412>
	<obo:IAO_0000119>If used for food additives, this descriptor refers to the European Commission food additive regulation according to the four Food Additive Directives: the EEC Framework Directive on Food Additives (89/107/EEC), the Directive on colours (94/36/EC), the Directive on sweeteners (94/35/EC) and the 'miscellaneous' Directive (95/2/EC) [http://ec.europa.eu/food/fs/sfp/flav_index_en.html] and/or Codex Alimentarius Commission General Standard for Food Additives (CODEX STAN 192) [http://www.codexalimentarius.net/download/standards/4/CXS_192e.pdf].

If used for food supplement substances, this descriptor refers to the European Commission regulation in general [http://ec.europa.eu/food/food/labellingnutrition/supplements/index_en.htm] and specifically to the EC Directive on the approximation of the laws of the Members States relating to food supplements (2002/46/EC) [http://eur-lex.europa.eu/LexUriServ/LexUriServ.do?uri=OJ:L:2002:183:0051:0057:EN:PDF].</obo:IAO_0000119>
	<owl:deprecated rdf:datatype="&xsd;boolean">true</owl:deprecated>
	<obo:IAO_0000114 rdf:resource="&obo;IAO_0000122"/>
	<rdfs:comment xml:lang="en">LanguaL curation note: This term is only kept for backward compatibility. DO NOT USE for new indexing.</rdfs:comment>
	<oboInOwl:hasDbXref>LANGUAL:B3066</oboInOwl:hasDbXref>
</owl:Class>

<owl:Class rdf:about="&obo;FOODON_03413165">
	<rdfs:label xml:lang="en">monosodium glutamate</rdfs:label>
	<rdfs:subClassOf rdf:resource="http://www.geneontology.org/formats/oboInOwl#ObsoleteClass"/>
	<obo:IAO_0000412>http://langual.org</obo:IAO_0000412>
	<owl:deprecated rdf:datatype="&xsd;boolean">true</owl:deprecated>
	<obo:IAO_0000114 rdf:resource="&obo;IAO_0000122"/>
	<rdfs:comment xml:lang="en">LanguaL curation note: This term is only kept for backward compatibility. DO NOT USE for new indexing.</rdfs:comment>
	<oboInOwl:hasDbXref>LANGUAL:B3165</oboInOwl:hasDbXref>
</owl:Class>

<owl:Class rdf:about="&obo;FOODON_03413206">
	<rdfs:label xml:lang="en">potassium chloride</rdfs:label>
	<rdfs:subClassOf rdf:resource="http://www.geneontology.org/formats/oboInOwl#ObsoleteClass"/>
	<obo:IAO_0000412>http://langual.org</obo:IAO_0000412>
	<owl:deprecated rdf:datatype="&xsd;boolean">true</owl:deprecated>
	<obo:IAO_0000114 rdf:resource="&obo;IAO_0000122"/>
	<rdfs:comment xml:lang="en">LanguaL curation note: This term is only kept for backward compatibility. DO NOT USE for new indexing.</rdfs:comment>
	<oboInOwl:hasDbXref>LANGUAL:B3206</oboInOwl:hasDbXref>
</owl:Class>

<owl:Class rdf:about="&obo;FOODON_03413256">
	<rdfs:label xml:lang="en">sodium hydrogen carbonate</rdfs:label>
	<rdfs:subClassOf rdf:resource="http://www.geneontology.org/formats/oboInOwl#ObsoleteClass"/>
	<obo:IAO_0000412>http://langual.org</obo:IAO_0000412>
	<owl:deprecated rdf:datatype="&xsd;boolean">true</owl:deprecated>
	<obo:IAO_0000114 rdf:resource="&obo;IAO_0000122"/>
	<rdfs:comment xml:lang="en">LanguaL curation note: This term is only kept for backward compatibility. DO NOT USE for new indexing.</rdfs:comment>
	<oboInOwl:hasDbXref>LANGUAL:B3256</oboInOwl:hasDbXref>
</owl:Class>

<owl:Class rdf:about="&obo;FOODON_03413412">
	<rdfs:label xml:lang="en">japanese-green</rdfs:label>
	<rdfs:subClassOf rdf:resource="http://www.geneontology.org/formats/oboInOwl#ObsoleteClass"/>
	<obo:IAO_0000412>http://langual.org</obo:IAO_0000412>
	<owl:deprecated rdf:datatype="&xsd;boolean">true</owl:deprecated>
	<obo:IAO_0000114 rdf:resource="&obo;IAO_0000122"/>
	<rdfs:comment xml:lang="en">LanguaL curation note: This term is only kept for backward compatibility. DO NOT USE for new indexing.</rdfs:comment>
	<oboInOwl:hasDbXref>LANGUAL:B3412</oboInOwl:hasDbXref>
</owl:Class>

<owl:Class rdf:about="&obo;FOODON_03414301">
	<rdfs:label xml:lang="en">mustard and cress</rdfs:label>
	<rdfs:subClassOf rdf:resource="http://www.geneontology.org/formats/oboInOwl#ObsoleteClass"/>
	<obo:IAO_0000412>http://langual.org</obo:IAO_0000412>
	<owl:deprecated rdf:datatype="&xsd;boolean">true</owl:deprecated>
	<obo:IAO_0000114 rdf:resource="&obo;IAO_0000122"/>
	<oboInOwl:hasDbXref>LANGUAL:B4301</oboInOwl:hasDbXref>
</owl:Class>

<owl:Class rdf:about="&obo;FOODON_03414352">
	<rdfs:label xml:lang="en">grains-of-paradise</rdfs:label>
	<rdfs:subClassOf rdf:resource="http://www.geneontology.org/formats/oboInOwl#ObsoleteClass"/>
	<obo:IAO_0000412>http://langual.org</obo:IAO_0000412>
	<obo:IAO_0000115 xml:lang="en">Descriptor inactivated due to duplication.




&lt;SCINAM&gt;Aframomum melegueta K.Schum. [EuroFIR-NETTOX 2007 4]

&lt;DICTION&gt;$i$Aframomum melegueta$/i$ is a species in the ginger family, $i$Zingiberaceae$/i$. This spice, commonly known as grains of paradise, melegueta pepper, alligator pepper, Guinea grains or Guinea pepper, is obtained from the ground seeds; it gives a pungent, peppery flavour.[http://en.wikipedia.org/wiki/Aframomum_melegueta]</obo:IAO_0000115>
	<obo:IAO_0000119>WIKIPEDIA:Aframomum_melegueta</obo:IAO_0000119>
	<owl:deprecated rdf:datatype="&xsd;boolean">true</owl:deprecated>
	<obo:IAO_0000114 rdf:resource="&obo;IAO_0000122"/>
	<rdfs:comment xml:lang="en">LanguaL curation note: This term is only kept for backward compatibility. DO NOT USE for new indexing.</rdfs:comment>
	<oboInOwl:hasDbXref>LANGUAL:B4352</oboInOwl:hasDbXref>
</owl:Class>

<owl:Class rdf:about="&obo;FOODON_03420001">
	<rdfs:label xml:lang="en">part of plant or animal not known</rdfs:label>
	<rdfs:subClassOf rdf:resource="http://www.geneontology.org/formats/oboInOwl#ObsoleteClass"/>
	<obo:IAO_0000412>http://langual.org</obo:IAO_0000412>
	<owl:deprecated rdf:datatype="&xsd;boolean">true</owl:deprecated>
	<obo:IAO_0000114 rdf:resource="&obo;IAO_0000122"/>
	<rdfs:comment xml:lang="en">LanguaL curation note: Used only in conjunction with *FOOD SOURCE NOT KNOWN*, i.e., if it is not known whether the food source is animal, plant, microorganism or chemical.</rdfs:comment>
	<oboInOwl:hasDbXref>LANGUAL:C0001</oboInOwl:hasDbXref>
</owl:Class>

<owl:Class rdf:about="&obo;FOODON_03420005">
	<rdfs:label xml:lang="en">part of plant or animal not applicable</rdfs:label>
	<rdfs:subClassOf rdf:resource="http://www.geneontology.org/formats/oboInOwl#ObsoleteClass"/>
	<obo:IAO_0000412>http://langual.org</obo:IAO_0000412>
	<owl:deprecated rdf:datatype="&xsd;boolean">true</owl:deprecated>
	<obo:IAO_0000114 rdf:resource="&obo;IAO_0000122"/>
	<rdfs:comment xml:lang="en">LanguaL curation note: Used only for chemical food products.</rdfs:comment>
	<oboInOwl:hasDbXref>LANGUAL:C0005</oboInOwl:hasDbXref>
</owl:Class>

<owl:Class rdf:about="&obo;FOODON_03420246">
	<rdfs:label xml:lang="en">ink, aquatic animal</rdfs:label>
	<rdfs:subClassOf rdf:resource="http://www.geneontology.org/formats/oboInOwl#ObsoleteClass"/>
	<obo:IAO_0000412>http://langual.org</obo:IAO_0000412>
	<owl:deprecated rdf:datatype="&xsd;boolean">true</owl:deprecated>
	<obo:IAO_0000114 rdf:resource="&obo;IAO_0000122"/>
	<oboInOwl:hasDbXref>LANGUAL:C0246</oboInOwl:hasDbXref>
</owl:Class>

<owl:Class rdf:about="&obo;FOODON_03430001">
	<rdfs:label xml:lang="en">physical state, shape or form not known</rdfs:label>
	<rdfs:subClassOf rdf:resource="http://www.geneontology.org/formats/oboInOwl#ObsoleteClass"/>
	<obo:IAO_0000412>http://langual.org</obo:IAO_0000412>
	<owl:deprecated rdf:datatype="&xsd;boolean">true</owl:deprecated>
	<obo:IAO_0000114 rdf:resource="&obo;IAO_0000122"/>
	<rdfs:comment xml:lang="en">LanguaL curation note: Used when nothing is known about the physical state, shape or form of the food product.</rdfs:comment>
	<oboInOwl:hasDbXref>LANGUAL:E0001</oboInOwl:hasDbXref>
</owl:Class>

<owl:Class rdf:about="&obo;FOODON_03430172">
	<rdfs:label xml:lang="en">supplement form, other</rdfs:label>
	<rdfs:subClassOf rdf:resource="http://www.geneontology.org/formats/oboInOwl#ObsoleteClass"/>
	<obo:IAO_0000412>http://langual.org</obo:IAO_0000412>
	<obo:IAO_0000115 xml:lang="en">Other liquid or powder forms for ingestion in dose amounts. Other forms not represented for use as a conventional food or as a sole item of a meal or the diet.</obo:IAO_0000115>
	<owl:deprecated rdf:datatype="&xsd;boolean">true</owl:deprecated>
	<obo:IAO_0000114 rdf:resource="&obo;IAO_0000122"/>
	<oboInOwl:hasDbXref>LANGUAL:E0172</oboInOwl:hasDbXref>
</owl:Class>

<owl:Class rdf:about="&obo;FOODON_03430177">
	<rdfs:label xml:lang="en">supplement form, unknown</rdfs:label>
	<rdfs:subClassOf rdf:resource="http://www.geneontology.org/formats/oboInOwl#ObsoleteClass"/>
	<obo:IAO_0000412>http://langual.org</obo:IAO_0000412>
	<owl:deprecated rdf:datatype="&xsd;boolean">true</owl:deprecated>
	<obo:IAO_0000114 rdf:resource="&obo;IAO_0000122"/>
	<rdfs:comment xml:lang="en">LanguaL curation note: Used when nothing is known about the form of the dietary supplement.</rdfs:comment>
	<oboInOwl:hasDbXref>LANGUAL:E0177</oboInOwl:hasDbXref>
</owl:Class>

<owl:Class rdf:about="&obo;FOODON_03440001">
	<rdfs:label xml:lang="en">extent of heat treatment not known</rdfs:label>
	<rdfs:subClassOf rdf:resource="http://www.geneontology.org/formats/oboInOwl#ObsoleteClass"/>
	<obo:IAO_0000412>http://langual.org</obo:IAO_0000412>
	<owl:deprecated rdf:datatype="&xsd;boolean">true</owl:deprecated>
	<obo:IAO_0000114 rdf:resource="&obo;IAO_0000122"/>
	<rdfs:comment xml:lang="en">LanguaL curation note: Used only when no information is available about the use of or degree of heat treatment performed.</rdfs:comment>
	<oboInOwl:hasDbXref>LANGUAL:F0001</oboInOwl:hasDbXref>
</owl:Class>

<owl:Class rdf:about="&obo;FOODON_03480001">
	<rdfs:label xml:lang="en">packing medium not known</rdfs:label>
	<rdfs:subClassOf rdf:resource="http://www.geneontology.org/formats/oboInOwl#ObsoleteClass"/>
	<obo:IAO_0000412>http://langual.org</obo:IAO_0000412>
	<owl:deprecated rdf:datatype="&xsd;boolean">true</owl:deprecated>
	<obo:IAO_0000114 rdf:resource="&obo;IAO_0000122"/>
	<rdfs:comment xml:lang="en">LanguaL curation note: Used when nothing is known about the packing medium, if any is present.</rdfs:comment>
	<oboInOwl:hasDbXref>LANGUAL:K0001</oboInOwl:hasDbXref>
</owl:Class>

<owl:Class rdf:about="&obo;FOODON_03480004">
	<rdfs:label xml:lang="en">packing medium, other</rdfs:label>
	<rdfs:subClassOf rdf:resource="http://www.geneontology.org/formats/oboInOwl#ObsoleteClass"/>
	<obo:IAO_0000412>http://langual.org</obo:IAO_0000412>
	<owl:deprecated rdf:datatype="&xsd;boolean">true</owl:deprecated>
	<obo:IAO_0000114 rdf:resource="&obo;IAO_0000122"/>
	<rdfs:comment xml:lang="en">LanguaL curation note: Used when the packing medium does not fall under any of the major categories listed.</rdfs:comment>
	<oboInOwl:hasDbXref>LANGUAL:K0004</oboInOwl:hasDbXref>
</owl:Class>

<owl:Class rdf:about="&obo;FOODON_03490001">
	<rdfs:label xml:lang="en">container or wrapping not known</rdfs:label>
	<rdfs:subClassOf rdf:resource="http://www.geneontology.org/formats/oboInOwl#ObsoleteClass"/>
	<obo:IAO_0000412>http://langual.org</obo:IAO_0000412>
	<owl:deprecated rdf:datatype="&xsd;boolean">true</owl:deprecated>
	<obo:IAO_0000114 rdf:resource="&obo;IAO_0000122"/>
	<rdfs:comment xml:lang="en">LanguaL curation note: Used when it is not known what container or wrapping, if any, is present.</rdfs:comment>
	<oboInOwl:hasDbXref>LANGUAL:M0001</oboInOwl:hasDbXref>
</owl:Class>

<owl:Class rdf:about="&obo;FOODON_03490003">
	<rdfs:label xml:lang="en">no container or wrapping used</rdfs:label>
	<rdfs:subClassOf rdf:resource="http://www.geneontology.org/formats/oboInOwl#ObsoleteClass"/>
	<obo:IAO_0000412>http://langual.org</obo:IAO_0000412>
	<owl:deprecated rdf:datatype="&xsd;boolean">true</owl:deprecated>
	<obo:IAO_0000114 rdf:resource="&obo;IAO_0000122"/>
	<rdfs:comment xml:lang="en">LanguaL curation note: Used when the food product is not packaged in a container or wrapping. includes products that are coated with a thin layer of wax, e.g., fruits or vegetables, but are not further packaged.</rdfs:comment>
	<oboInOwl:hasDbXref>LANGUAL:M0003</oboInOwl:hasDbXref>
</owl:Class>

<owl:Class rdf:about="&obo;FOODON_03490004">
	<rdfs:label xml:lang="en">container or wrapping, other</rdfs:label>
	<rdfs:subClassOf rdf:resource="http://www.geneontology.org/formats/oboInOwl#ObsoleteClass"/>
	<obo:IAO_0000412>http://langual.org</obo:IAO_0000412>
	<owl:deprecated rdf:datatype="&xsd;boolean">true</owl:deprecated>
	<obo:IAO_0000114 rdf:resource="&obo;IAO_0000122"/>
	<rdfs:comment xml:lang="en">LanguaL curation note: Used when the container does not fall under any of the major types listed.</rdfs:comment>
	<oboInOwl:hasDbXref>LANGUAL:M0004</oboInOwl:hasDbXref>
</owl:Class>

<owl:Class rdf:about="&obo;FOODON_03500001">
	<rdfs:label xml:lang="en">food contact surface not known</rdfs:label>
	<rdfs:subClassOf rdf:resource="http://www.geneontology.org/formats/oboInOwl#ObsoleteClass"/>
	<obo:IAO_0000412>http://langual.org</obo:IAO_0000412>
	<owl:deprecated rdf:datatype="&xsd;boolean">true</owl:deprecated>
	<obo:IAO_0000114 rdf:resource="&obo;IAO_0000122"/>
	<rdfs:comment xml:lang="en">LanguaL curation note: Used when it is not known what the food contact surface is, if any.</rdfs:comment>
	<oboInOwl:hasDbXref>LANGUAL:N0001</oboInOwl:hasDbXref>
</owl:Class>

<owl:Class rdf:about="&obo;FOODON_03500003">
	<rdfs:label xml:lang="en">no food contact surface present</rdfs:label>
	<rdfs:subClassOf rdf:resource="http://www.geneontology.org/formats/oboInOwl#ObsoleteClass"/>
	<obo:IAO_0000412>http://langual.org</obo:IAO_0000412>
	<owl:deprecated rdf:datatype="&xsd;boolean">true</owl:deprecated>
	<obo:IAO_0000114 rdf:resource="&obo;IAO_0000122"/>
	<rdfs:comment xml:lang="en">LanguaL curation note: Used when the product is neither packed nor coated with a protective coating.</rdfs:comment>
	<oboInOwl:hasDbXref>LANGUAL:N0003</oboInOwl:hasDbXref>
</owl:Class>

<owl:Class rdf:about="&obo;FOODON_03500004">
	<rdfs:label xml:lang="en">food contact surface, other</rdfs:label>
	<rdfs:subClassOf rdf:resource="http://www.geneontology.org/formats/oboInOwl#ObsoleteClass"/>
	<obo:IAO_0000412>http://langual.org</obo:IAO_0000412>
	<owl:deprecated rdf:datatype="&xsd;boolean">true</owl:deprecated>
	<obo:IAO_0000114 rdf:resource="&obo;IAO_0000122"/>
	<rdfs:comment xml:lang="en">LanguaL curation note: Used only if the contact surface does not fall under any of the major types listed.</rdfs:comment>
	<oboInOwl:hasDbXref>LANGUAL:N0004</oboInOwl:hasDbXref>
</owl:Class>

<owl:Class rdf:about="&obo;FOODON_03510001">
	<rdfs:label xml:lang="en">consumer group not known</rdfs:label>
	<rdfs:subClassOf rdf:resource="http://www.geneontology.org/formats/oboInOwl#ObsoleteClass"/>
	<obo:IAO_0000412>http://langual.org</obo:IAO_0000412>
	<owl:deprecated rdf:datatype="&xsd;boolean">true</owl:deprecated>
	<obo:IAO_0000114 rdf:resource="&obo;IAO_0000122"/>
	<rdfs:comment xml:lang="en">LanguaL curation note: Used when nothing is know about the consumer group.</rdfs:comment>
	<oboInOwl:hasDbXref>LANGUAL:P0001</oboInOwl:hasDbXref>
</owl:Class>

<owl:Class rdf:about="&obo;FOODON_03510003">
	<rdfs:label xml:lang="en">consumer group not applicable</rdfs:label>
	<rdfs:subClassOf rdf:resource="http://www.geneontology.org/formats/oboInOwl#ObsoleteClass"/>
	<obo:IAO_0000412>http://langual.org</obo:IAO_0000412>
	<owl:deprecated rdf:datatype="&xsd;boolean">true</owl:deprecated>
	<obo:IAO_0000114 rdf:resource="&obo;IAO_0000122"/>
	<oboInOwl:hasDbXref>LANGUAL:P0003</oboInOwl:hasDbXref>
</owl:Class>

<owl:Class rdf:about="&obo;FOODON_03510024">
	<rdfs:label xml:lang="en">human consumer, no age specification</rdfs:label>
	<rdfs:subClassOf rdf:resource="http://www.geneontology.org/formats/oboInOwl#ObsoleteClass"/>
	<obo:IAO_0000412>http://langual.org</obo:IAO_0000412>
	<obo:IAO_0000115 xml:lang="en">Food produced and marketed for human use without any restriction by age.</obo:IAO_0000115>
	<owl:deprecated rdf:datatype="&xsd;boolean">true</owl:deprecated>
	<obo:IAO_0000114 rdf:resource="&obo;IAO_0000122"/>
	<obo:IAO_0100001 rdf:resource="&obo;FOODON_03510026"/>
	<oboInOwl:hasSynonym xml:lang="en">all ages</oboInOwl:hasSynonym>
	<oboInOwl:hasDbXref>LANGUAL:P0024</oboInOwl:hasDbXref>
</owl:Class>

<owl:Class rdf:about="&obo;FOODON_03510160">
	<rdfs:label xml:lang="en">label or labeling claim</rdfs:label>
	<rdfs:subClassOf rdf:resource="http://www.geneontology.org/formats/oboInOwl#ObsoleteClass"/>
	<obo:IAO_0000412>http://langual.org</obo:IAO_0000412>
	<obo:IAO_0000115 xml:lang="en">Use these descriptors when indexing food names for which label or labeling information is available. 'Labeling' includes all labels and other written, printed or graphic material that appears on a product's container or wrapping, as well as any such material accompanying a product.</obo:IAO_0000115>
	<owl:deprecated rdf:datatype="&xsd;boolean">true</owl:deprecated>
	<obo:IAO_0000114 rdf:resource="&obo;IAO_0000122"/>
	<rdfs:comment xml:lang="en">LanguaL curation note: This term is only kept for backward compatibility. DO NOT USE for new indexing.</rdfs:comment>
	<oboInOwl:hasDbXref>LANGUAL:P0160</oboInOwl:hasDbXref>
</owl:Class>

<owl:Class rdf:about="&obo;FOODON_03510163">
	<rdfs:label xml:lang="en">labeling claim</rdfs:label>
	<rdfs:subClassOf rdf:resource="http://www.geneontology.org/formats/oboInOwl#ObsoleteClass"/>
	<obo:IAO_0000412>http://langual.org</obo:IAO_0000412>
	<obo:IAO_0000115 xml:lang="en">Use when the 'claim or use' index term is derived from written, printed or graphic material that appears on a product's container or wrapping but is not a part of the food label.</obo:IAO_0000115>
	<owl:deprecated rdf:datatype="&xsd;boolean">true</owl:deprecated>
	<obo:IAO_0000114 rdf:resource="&obo;IAO_0000122"/>
	<rdfs:comment xml:lang="en">LanguaL curation note: This term is only kept for backward compatibility. DO NOT USE for new indexing.</rdfs:comment>
	<oboInOwl:hasDbXref>LANGUAL:P0163</oboInOwl:hasDbXref>
</owl:Class>

<owl:Class rdf:about="&obo;FOODON_03510258">
	<rdfs:label xml:lang="en">human consumer, other</rdfs:label>
	<rdfs:subClassOf rdf:resource="http://www.geneontology.org/formats/oboInOwl#ObsoleteClass"/>
	<obo:IAO_0000412>http://langual.org</obo:IAO_0000412>
	<owl:deprecated rdf:datatype="&xsd;boolean">true</owl:deprecated>
	<obo:IAO_0000114 rdf:resource="&obo;IAO_0000122"/>
	<oboInOwl:hasDbXref>LANGUAL:P0258</oboInOwl:hasDbXref>
</owl:Class>

<owl:Class rdf:about="&obo;FOODON_03530001">
	<rdfs:label xml:lang="en">adjunct characteristics of food not known</rdfs:label>
	<rdfs:subClassOf rdf:resource="http://www.geneontology.org/formats/oboInOwl#ObsoleteClass"/>
	<obo:IAO_0000412>http://langual.org</obo:IAO_0000412>
	<owl:deprecated rdf:datatype="&xsd;boolean">true</owl:deprecated>
	<obo:IAO_0000114 rdf:resource="&obo;IAO_0000122"/>
	<oboInOwl:hasDbXref>LANGUAL:Z0001</oboInOwl:hasDbXref>
</owl:Class>

<owl:Class rdf:about="&obo;FOODON_03530003">
	<rdfs:label xml:lang="en">meat color, undesignated or unknown</rdfs:label>
	<rdfs:subClassOf rdf:resource="http://www.geneontology.org/formats/oboInOwl#ObsoleteClass"/>
	<obo:IAO_0000412>http://langual.org</obo:IAO_0000412>
	<owl:deprecated rdf:datatype="&xsd;boolean">true</owl:deprecated>
	<obo:IAO_0000114 rdf:resource="&obo;IAO_0000122"/>
	<rdfs:comment xml:lang="en">LanguaL curation note: Used only for poultry meat that comes from the back, the neck or for which the color is not known.</rdfs:comment>
	<oboInOwl:hasSynonym xml:lang="en">back meat, poultry</oboInOwl:hasSynonym>
	<oboInOwl:hasSynonym xml:lang="en">neck meat, poultry</oboInOwl:hasSynonym>
	<oboInOwl:hasDbXref>LANGUAL:Z0003</oboInOwl:hasDbXref>
</owl:Class>

<owl:Class rdf:about="&obo;FOODON_03530018">
	<rdfs:label xml:lang="en">cut of meat not known</rdfs:label>
	<rdfs:subClassOf rdf:resource="http://www.geneontology.org/formats/oboInOwl#ObsoleteClass"/>
	<obo:IAO_0000412>http://langual.org</obo:IAO_0000412>
	<owl:deprecated rdf:datatype="&xsd;boolean">true</owl:deprecated>
	<obo:IAO_0000114 rdf:resource="&obo;IAO_0000122"/>
	<oboInOwl:hasDbXref>LANGUAL:Z0018</oboInOwl:hasDbXref>
</owl:Class>

<owl:Class rdf:about="&obo;FOODON_03530019">
	<rdfs:label xml:lang="en">grade of meat not known</rdfs:label>
	<rdfs:subClassOf rdf:resource="http://www.geneontology.org/formats/oboInOwl#ObsoleteClass"/>
	<obo:IAO_0000412>http://langual.org</obo:IAO_0000412>
	<owl:deprecated rdf:datatype="&xsd;boolean">true</owl:deprecated>
	<obo:IAO_0000114 rdf:resource="&obo;IAO_0000122"/>
	<oboInOwl:hasDbXref>LANGUAL:Z0019</oboInOwl:hasDbXref>
</owl:Class>

<owl:Class rdf:about="&obo;FOODON_03530048">
	<rdfs:label xml:lang="en">cut of meat, other</rdfs:label>
	<rdfs:subClassOf rdf:resource="http://www.geneontology.org/formats/oboInOwl#ObsoleteClass"/>
	<obo:IAO_0000412>http://langual.org</obo:IAO_0000412>
	<owl:deprecated rdf:datatype="&xsd;boolean">true</owl:deprecated>
	<obo:IAO_0000114 rdf:resource="&obo;IAO_0000122"/>
	<oboInOwl:hasDbXref>LANGUAL:Z0048</oboInOwl:hasDbXref>
</owl:Class>

<owl:Class rdf:about="&obo;FOODON_03530061">
	<rdfs:label xml:lang="en">color of fish flesh not known</rdfs:label>
	<rdfs:subClassOf rdf:resource="http://www.geneontology.org/formats/oboInOwl#ObsoleteClass"/>
	<obo:IAO_0000412>http://langual.org</obo:IAO_0000412>
	<owl:deprecated rdf:datatype="&xsd;boolean">true</owl:deprecated>
	<obo:IAO_0000114 rdf:resource="&obo;IAO_0000122"/>
	<oboInOwl:hasDbXref>LANGUAL:Z0061</oboInOwl:hasDbXref>
</owl:Class>

<owl:Class rdf:about="&obo;FOODON_03530095">
	<rdfs:label xml:lang="en">sausage casing not known</rdfs:label>
	<rdfs:subClassOf rdf:resource="http://www.geneontology.org/formats/oboInOwl#ObsoleteClass"/>
	<obo:IAO_0000412>http://langual.org</obo:IAO_0000412>
	<owl:deprecated rdf:datatype="&xsd;boolean">true</owl:deprecated>
	<obo:IAO_0000114 rdf:resource="&obo;IAO_0000122"/>
	<oboInOwl:hasDbXref>LANGUAL:Z0095</oboInOwl:hasDbXref>
</owl:Class>

<owl:Class rdf:about="&obo;FOODON_03530205">
	<rdfs:label xml:lang="en">maturity or ripeness unknown</rdfs:label>
	<rdfs:subClassOf rdf:resource="http://www.geneontology.org/formats/oboInOwl#ObsoleteClass"/>
	<obo:IAO_0000412>http://langual.org</obo:IAO_0000412>
	<owl:deprecated rdf:datatype="&xsd;boolean">true</owl:deprecated>
	<obo:IAO_0000114 rdf:resource="&obo;IAO_0000122"/>
	<oboInOwl:hasDbXref>LANGUAL:Z0205</oboInOwl:hasDbXref>
</owl:Class>

<owl:Class rdf:about="&obo;FOODON_03530215">
	<rdfs:label xml:lang="en">production environment not known</rdfs:label>
	<rdfs:subClassOf rdf:resource="http://www.geneontology.org/formats/oboInOwl#ObsoleteClass"/>
	<obo:IAO_0000412>http://langual.org</obo:IAO_0000412>
	<owl:deprecated rdf:datatype="&xsd;boolean">true</owl:deprecated>
	<obo:IAO_0000114 rdf:resource="&obo;IAO_0000122"/>
	<oboInOwl:hasDbXref>LANGUAL:Z0215</oboInOwl:hasDbXref>
</owl:Class>

<owl:Class rdf:about="&obo;FOODON_03530216">
	<rdfs:label xml:lang="en">production environment other</rdfs:label>
	<rdfs:subClassOf rdf:resource="http://www.geneontology.org/formats/oboInOwl#ObsoleteClass"/>
	<obo:IAO_0000412>http://langual.org</obo:IAO_0000412>
	<owl:deprecated rdf:datatype="&xsd;boolean">true</owl:deprecated>
	<obo:IAO_0000114 rdf:resource="&obo;IAO_0000122"/>
	<oboInOwl:hasDbXref>LANGUAL:Z0216</oboInOwl:hasDbXref>
</owl:Class>

<owl:Class rdf:about="&obo;FOODON_03530262">
	<rdfs:label xml:lang="en">food content range, other</rdfs:label>
	<rdfs:subClassOf rdf:resource="http://www.geneontology.org/formats/oboInOwl#ObsoleteClass"/>
	<obo:IAO_0000412>http://langual.org</obo:IAO_0000412>
	<owl:deprecated rdf:datatype="&xsd;boolean">true</owl:deprecated>
	<obo:IAO_0000114 rdf:resource="&obo;IAO_0000122"/>
	<rdfs:comment xml:lang="en">LanguaL curation note: This term is for CLASSIFICATION ONLY; DO NOT USE term in indexing. Use a more precise narrower term.</rdfs:comment>
	<oboInOwl:hasDbXref>LANGUAL:Z0262</oboInOwl:hasDbXref>
</owl:Class>

<owl:Class rdf:about="&obo;FOODON_03520001">
	<rdfs:label xml:lang="en">geographic place or region not known</rdfs:label>
	<rdfs:subClassOf rdf:resource="http://www.geneontology.org/formats/oboInOwl#ObsoleteClass"/>
	<obo:IAO_0000412>http://langual.org</obo:IAO_0000412>
	<owl:deprecated rdf:datatype="&xsd;boolean">true</owl:deprecated>
	<obo:IAO_0000114 rdf:resource="&obo;IAO_0000122"/>
	<oboInOwl:hasDbXref>LANGUAL:R0001</oboInOwl:hasDbXref>
</owl:Class>

<owl:Class rdf:about="&obo;FOODON_03520199">
	<rdfs:label xml:lang="en">czechoslovakia</rdfs:label>
	<rdfs:subClassOf rdf:resource="http://www.geneontology.org/formats/oboInOwl#ObsoleteClass"/>
	<obo:IAO_0000412>http://langual.org</obo:IAO_0000412>
	<owl:deprecated rdf:datatype="&xsd;boolean">true</owl:deprecated>
	<obo:IAO_0000114 rdf:resource="&obo;IAO_0000122"/>
	<rdfs:comment xml:lang="en">LanguaL curation note: This term is only kept for backward compatibility. DO NOT USE for new indexing.</rdfs:comment>
	<oboInOwl:hasDbXref>LANGUAL:R0199</oboInOwl:hasDbXref>
</owl:Class></rdf:RDF>