<?xml version="1.0"?>
<rdf:RDF xmlns="http://purl.obolibrary.org/obo/foodon/imports/langual_deprecated_import.owl#"
     xml:base="http://purl.obolibrary.org/obo/foodon/imports/langual_deprecated_import.owl"
     xmlns:rdf="http://www.w3.org/1999/02/22-rdf-syntax-ns#"
     xmlns:owl="http://www.w3.org/2002/07/owl#"
     xmlns:oboInOwl="http://www.geneontology.org/formats/oboInOwl#"
     xmlns:xml="http://www.w3.org/XML/1998/namespace"
     xmlns:xsd="http://www.w3.org/2001/XMLSchema#"
     xmlns:Lt="&amp;lt;"
     xmlns:taxon="http://purl.obolibrary.org/obo/NCBITaxon#"
     xmlns:rdfs="http://www.w3.org/2000/01/rdf-schema#"
     xmlns:obo="http://purl.obolibrary.org/obo/"
     xmlns:Gt="&amp;gt;"
     xmlns:dc="http://purl.org/dc/elements/1.1/">
    <owl:Ontology rdf:about="http://purl.obolibrary.org/obo/foodon/imports/langual_deprecated_import.owl">
        <dc:contributor xml:lang="en">Damion Dooley</dc:contributor>
    </owl:Ontology>
    


    <!-- 
    ///////////////////////////////////////////////////////////////////////////////////////
    //
    // Annotation properties
    //
    ///////////////////////////////////////////////////////////////////////////////////////
     -->

    


    <!-- http://purl.obolibrary.org/obo/IAO_0000114 -->

    <owl:AnnotationProperty rdf:about="http://purl.obolibrary.org/obo/IAO_0000114"/>
    


    <!-- http://purl.obolibrary.org/obo/IAO_0000115 -->

    <owl:AnnotationProperty rdf:about="http://purl.obolibrary.org/obo/IAO_0000115"/>
    


    <!-- http://purl.obolibrary.org/obo/IAO_0000119 -->

    <owl:AnnotationProperty rdf:about="http://purl.obolibrary.org/obo/IAO_0000119"/>
    


    <!-- http://purl.obolibrary.org/obo/IAO_0000231 -->

    <owl:AnnotationProperty rdf:about="http://purl.obolibrary.org/obo/IAO_0000231"/>
    


    <!-- http://purl.obolibrary.org/obo/IAO_0000412 -->

    <owl:AnnotationProperty rdf:about="http://purl.obolibrary.org/obo/IAO_0000412"/>
    


    <!-- http://purl.obolibrary.org/obo/IAO_0100001 -->

    <owl:AnnotationProperty rdf:about="http://purl.obolibrary.org/obo/IAO_0100001"/>
    


    <!-- http://www.geneontology.org/formats/oboInOwl#hasBroadSynonym -->

    <owl:AnnotationProperty rdf:about="http://www.geneontology.org/formats/oboInOwl#hasBroadSynonym"/>
    


    <!-- http://www.geneontology.org/formats/oboInOwl#hasDbXref -->

    <owl:AnnotationProperty rdf:about="http://www.geneontology.org/formats/oboInOwl#hasDbXref"/>
    


    <!-- http://www.geneontology.org/formats/oboInOwl#hasNarrowSynonym -->

    <owl:AnnotationProperty rdf:about="http://www.geneontology.org/formats/oboInOwl#hasNarrowSynonym"/>
    


    <!-- http://www.geneontology.org/formats/oboInOwl#hasSynonym -->

    <owl:AnnotationProperty rdf:about="http://www.geneontology.org/formats/oboInOwl#hasSynonym"/>
    


    <!-- 
    ///////////////////////////////////////////////////////////////////////////////////////
    //
    // Object Properties
    //
    ///////////////////////////////////////////////////////////////////////////////////////
     -->

    


    <!-- http://purl.obolibrary.org/obo/RO_0000087 -->

    <owl:ObjectProperty rdf:about="http://purl.obolibrary.org/obo/RO_0000087"/>
    


    <!-- 
    ///////////////////////////////////////////////////////////////////////////////////////
    //
    // Classes
    //
    ///////////////////////////////////////////////////////////////////////////////////////
     -->

    


    <!-- http://purl.obolibrary.org/obo/FOODON_03400000 -->

    <owl:Class rdf:about="http://purl.obolibrary.org/obo/FOODON_03400000">
        <rdfs:subClassOf rdf:resource="http://www.geneontology.org/formats/oboInOwl#ObsoleteClass"/>
        <obo:IAO_0000115 xml:lang="en">2014</obo:IAO_0000115>
        <obo:IAO_0000412>http://langual.org</obo:IAO_0000412>
        <oboInOwl:hasDbXref>LANGUAL:00000</oboInOwl:hasDbXref>
        <rdfs:label xml:lang="en">langual thesaurus root (deprecated)</rdfs:label>
        <owl:deprecated rdf:datatype="http://www.w3.org/2001/XMLSchema#boolean">true</owl:deprecated>
    </owl:Class>
    


    <!-- http://purl.obolibrary.org/obo/FOODON_03410001 -->

    <owl:Class rdf:about="http://purl.obolibrary.org/obo/FOODON_03410001">
        <rdfs:subClassOf rdf:resource="http://www.geneontology.org/formats/oboInOwl#ObsoleteClass"/>
        <obo:IAO_0000412>http://langual.org</obo:IAO_0000412>
        <oboInOwl:hasDbXref>LANGUAL:B0001</oboInOwl:hasDbXref>
        <rdfs:comment xml:lang="en">LanguaL curation note: Used only if so little is known about the food source that not even *ANIMAL USED AS FOOD SOURCE*, *PLANT USED AS FOOD SOURCE*, *ALGAE OR FUNGUS AS FOOD SOURCE* or *CHEMICAL FOOD SOURCE* can be assigned.</rdfs:comment>
        <rdfs:label xml:lang="en">food source not known (deprecated)</rdfs:label>
        <owl:deprecated rdf:datatype="http://www.w3.org/2001/XMLSchema#boolean">true</owl:deprecated>
    </owl:Class>
    


    <!-- http://purl.obolibrary.org/obo/FOODON_03411000 -->

    <owl:Class rdf:about="http://purl.obolibrary.org/obo/FOODON_03411000">
        <rdfs:subClassOf rdf:resource="http://www.geneontology.org/formats/oboInOwl#ObsoleteClass"/>
        <obo:IAO_0000412>http://langual.org</obo:IAO_0000412>
        <oboInOwl:hasDbXref>LANGUAL:B1000</oboInOwl:hasDbXref>
        <rdfs:label xml:lang="en">cattle and swine and calf (deprecated)</rdfs:label>
        <owl:deprecated rdf:datatype="http://www.w3.org/2001/XMLSchema#boolean">true</owl:deprecated>
    </owl:Class>
    


    <!-- http://purl.obolibrary.org/obo/FOODON_03411028 -->

    <owl:Class rdf:about="http://purl.obolibrary.org/obo/FOODON_03411028">
        <rdfs:subClassOf rdf:resource="http://www.geneontology.org/formats/oboInOwl#ObsoleteClass"/>
        <obo:IAO_0000412>http://langual.org</obo:IAO_0000412>
        <oboInOwl:hasDbXref>LANGUAL:B1028</oboInOwl:hasDbXref>
        <rdfs:label xml:lang="en">grapefruit and orange (deprecated)</rdfs:label>
        <owl:deprecated rdf:datatype="http://www.w3.org/2001/XMLSchema#boolean">true</owl:deprecated>
    </owl:Class>
    


    <!-- http://purl.obolibrary.org/obo/FOODON_03411032 -->

    <owl:Class rdf:about="http://purl.obolibrary.org/obo/FOODON_03411032">
        <rdfs:subClassOf rdf:resource="http://www.geneontology.org/formats/oboInOwl#ObsoleteClass"/>
        <obo:IAO_0000412>http://langual.org</obo:IAO_0000412>
        <oboInOwl:hasDbXref>LANGUAL:B1032</oboInOwl:hasDbXref>
        <rdfs:label xml:lang="en">sole, species not known (deprecated)</rdfs:label>
        <owl:deprecated rdf:datatype="http://www.w3.org/2001/XMLSchema#boolean">true</owl:deprecated>
    </owl:Class>
    


    <!-- http://purl.obolibrary.org/obo/FOODON_03411105 -->

    <owl:Class rdf:about="http://purl.obolibrary.org/obo/FOODON_03411105">
        <rdfs:subClassOf rdf:resource="http://www.geneontology.org/formats/oboInOwl#ObsoleteClass"/>
        <obo:IAO_0000412>http://langual.org</obo:IAO_0000412>
        <oboInOwl:hasDbXref>LANGUAL:B1105</oboInOwl:hasDbXref>
        <rdfs:label xml:lang="en">cattle and swine (deprecated)</rdfs:label>
        <owl:deprecated rdf:datatype="http://www.w3.org/2001/XMLSchema#boolean">true</owl:deprecated>
    </owl:Class>
    


    <!-- http://purl.obolibrary.org/obo/FOODON_03411207 -->

    <owl:Class rdf:about="http://purl.obolibrary.org/obo/FOODON_03411207">
        <rdfs:subClassOf rdf:resource="http://www.geneontology.org/formats/oboInOwl#ObsoleteClass"/>
        <obo:IAO_0000412>http://langual.org</obo:IAO_0000412>
        <oboInOwl:hasDbXref>LANGUAL:B1207</oboInOwl:hasDbXref>
        <rdfs:comment xml:lang="en">LanguaL curation note: This term is only kept for backward compatibility. DO NOT USE for new indexing.</rdfs:comment>
        <rdfs:label xml:lang="en">prune (deprecated)</rdfs:label>
        <owl:deprecated rdf:datatype="http://www.w3.org/2001/XMLSchema#boolean">true</owl:deprecated>
    </owl:Class>
    


    <!-- http://purl.obolibrary.org/obo/FOODON_03411246 -->

    <owl:Class rdf:about="http://purl.obolibrary.org/obo/FOODON_03411246">
        <rdfs:subClassOf rdf:resource="http://www.geneontology.org/formats/oboInOwl#ObsoleteClass"/>
        <obo:IAO_0000412>http://langual.org</obo:IAO_0000412>
        <oboInOwl:hasDbXref>LANGUAL:B1246</oboInOwl:hasDbXref>
        <rdfs:label xml:lang="en">pineapple and grapefruit (deprecated)</rdfs:label>
        <owl:deprecated rdf:datatype="http://www.w3.org/2001/XMLSchema#boolean">true</owl:deprecated>
    </owl:Class>
    


    <!-- http://purl.obolibrary.org/obo/FOODON_03411321 -->

    <owl:Class rdf:about="http://purl.obolibrary.org/obo/FOODON_03411321">
        <rdfs:subClassOf rdf:resource="http://www.geneontology.org/formats/oboInOwl#ObsoleteClass"/>
        <obo:IAO_0000412>http://langual.org</obo:IAO_0000412>
        <oboInOwl:hasDbXref>LANGUAL:B1321</oboInOwl:hasDbXref>
        <rdfs:comment xml:lang="en">LanguaL curation note: This term is only kept for backward compatibility. DO NOT USE for new indexing.</rdfs:comment>
        <rdfs:label xml:lang="en">mace (deprecated)</rdfs:label>
        <owl:deprecated rdf:datatype="http://www.w3.org/2001/XMLSchema#boolean">true</owl:deprecated>
    </owl:Class>
    


    <!-- http://purl.obolibrary.org/obo/FOODON_03411424 -->

    <owl:Class rdf:about="http://purl.obolibrary.org/obo/FOODON_03411424">
        <rdfs:subClassOf rdf:resource="http://www.geneontology.org/formats/oboInOwl#ObsoleteClass"/>
        <obo:IAO_0000115 xml:lang="en">Synonym of *WALLEYE PIKE [B1398]*.</obo:IAO_0000115>
        <obo:IAO_0000412>http://langual.org</obo:IAO_0000412>
        <oboInOwl:hasDbXref>LANGUAL:B1424</oboInOwl:hasDbXref>
        <rdfs:comment xml:lang="en">LanguaL curation note: This term is only kept for backward compatibility. DO NOT USE for new indexing.</rdfs:comment>
        <rdfs:label xml:lang="en">blue pike (deprecated)</rdfs:label>
        <owl:deprecated rdf:datatype="http://www.w3.org/2001/XMLSchema#boolean">true</owl:deprecated>
    </owl:Class>
    


    <!-- http://purl.obolibrary.org/obo/FOODON_03411525 -->

    <owl:Class rdf:about="http://purl.obolibrary.org/obo/FOODON_03411525">
        <rdfs:subClassOf rdf:resource="http://www.geneontology.org/formats/oboInOwl#ObsoleteClass"/>
        <obo:IAO_0000412>http://langual.org</obo:IAO_0000412>
        <oboInOwl:hasDbXref>LANGUAL:B1525</oboInOwl:hasDbXref>
        <rdfs:label xml:lang="en">peanut with other nut or seed (deprecated)</rdfs:label>
        <owl:deprecated rdf:datatype="http://www.w3.org/2001/XMLSchema#boolean">true</owl:deprecated>
    </owl:Class>
    


    <!-- http://purl.obolibrary.org/obo/FOODON_03411526 -->

    <owl:Class rdf:about="http://purl.obolibrary.org/obo/FOODON_03411526">
        <rdfs:subClassOf rdf:resource="http://www.geneontology.org/formats/oboInOwl#ObsoleteClass"/>
        <obo:IAO_0000412>http://langual.org</obo:IAO_0000412>
        <obo:IAO_0100001 rdf:resource="http://purl.obolibrary.org/obo/FOODON_03412375"/>
        <oboInOwl:hasDbXref>LANGUAL:B1526</oboInOwl:hasDbXref>
        <rdfs:comment xml:lang="en">LanguaL curation note: This term is only kept for backward compatibility. DO NOT USE for new indexing.</rdfs:comment>
        <rdfs:label xml:lang="en">weakfish (deprecated)</rdfs:label>
        <owl:deprecated rdf:datatype="http://www.w3.org/2001/XMLSchema#boolean">true</owl:deprecated>
    </owl:Class>
    


    <!-- http://purl.obolibrary.org/obo/FOODON_03411605 -->

    <owl:Class rdf:about="http://purl.obolibrary.org/obo/FOODON_03411605">
        <rdfs:subClassOf rdf:resource="http://www.geneontology.org/formats/oboInOwl#ObsoleteClass"/>
        <obo:IAO_0000412>http://langual.org</obo:IAO_0000412>
        <oboInOwl:hasDbXref>LANGUAL:B1605</oboInOwl:hasDbXref>
        <rdfs:label xml:lang="en">pea and onion (deprecated)</rdfs:label>
        <owl:deprecated rdf:datatype="http://www.w3.org/2001/XMLSchema#boolean">true</owl:deprecated>
    </owl:Class>
    


    <!-- http://purl.obolibrary.org/obo/FOODON_03411613 -->

    <owl:Class rdf:about="http://purl.obolibrary.org/obo/FOODON_03411613">
        <rdfs:subClassOf rdf:resource="http://www.geneontology.org/formats/oboInOwl#ObsoleteClass"/>
        <obo:IAO_0000412>http://langual.org</obo:IAO_0000412>
        <oboInOwl:hasDbXref>LANGUAL:B1613</oboInOwl:hasDbXref>
        <rdfs:label xml:lang="en">pea and carrot (deprecated)</rdfs:label>
        <owl:deprecated rdf:datatype="http://www.w3.org/2001/XMLSchema#boolean">true</owl:deprecated>
    </owl:Class>
    


    <!-- http://purl.obolibrary.org/obo/FOODON_03411619 -->

    <owl:Class rdf:about="http://purl.obolibrary.org/obo/FOODON_03411619">
        <rdfs:subClassOf rdf:resource="http://www.geneontology.org/formats/oboInOwl#ObsoleteClass"/>
        <obo:IAO_0000231 xml:lang="en">Duplicate entry.</obo:IAO_0000231>
        <obo:IAO_0000412>http://langual.org</obo:IAO_0000412>
        <oboInOwl:hasDbXref>LANGUAL:B1619</oboInOwl:hasDbXref>
        <rdfs:comment xml:lang="en">LanguaL curation note: This term is only kept for backward compatibility. DO NOT USE for new indexing.</rdfs:comment>
        <rdfs:label xml:lang="en">reindeer (deprecated)</rdfs:label>
        <owl:deprecated rdf:datatype="http://www.w3.org/2001/XMLSchema#boolean">true</owl:deprecated>
    </owl:Class>
    


    <!-- http://purl.obolibrary.org/obo/FOODON_03411631 -->

    <owl:Class rdf:about="http://purl.obolibrary.org/obo/FOODON_03411631">
        <rdfs:subClassOf rdf:resource="http://www.geneontology.org/formats/oboInOwl#ObsoleteClass"/>
        <obo:IAO_0000412>http://langual.org</obo:IAO_0000412>
        <oboInOwl:hasDbXref>LANGUAL:B1631</oboInOwl:hasDbXref>
        <rdfs:label xml:lang="en">pineapple and orange (deprecated)</rdfs:label>
        <owl:deprecated rdf:datatype="http://www.w3.org/2001/XMLSchema#boolean">true</owl:deprecated>
    </owl:Class>
    


    <!-- http://purl.obolibrary.org/obo/FOODON_03411680 -->

    <owl:Class rdf:about="http://purl.obolibrary.org/obo/FOODON_03411680">
        <rdfs:subClassOf rdf:resource="http://www.geneontology.org/formats/oboInOwl#ObsoleteClass"/>
        <obo:IAO_0000412>http://langual.org</obo:IAO_0000412>
        <oboInOwl:hasDbXref>LANGUAL:B1680</oboInOwl:hasDbXref>
        <rdfs:label xml:lang="en">sugar cane and field corn (deprecated)</rdfs:label>
        <owl:deprecated rdf:datatype="http://www.w3.org/2001/XMLSchema#boolean">true</owl:deprecated>
    </owl:Class>
    


    <!-- http://purl.obolibrary.org/obo/FOODON_03411709 -->

    <owl:Class rdf:about="http://purl.obolibrary.org/obo/FOODON_03411709">
        <rdfs:subClassOf rdf:resource="http://www.geneontology.org/formats/oboInOwl#ObsoleteClass"/>
        <obo:IAO_0000412>http://langual.org</obo:IAO_0000412>
        <oboInOwl:hasDbXref>LANGUAL:B1709</oboInOwl:hasDbXref>
        <rdfs:label xml:lang="en">orange and apricot (deprecated)</rdfs:label>
        <owl:deprecated rdf:datatype="http://www.w3.org/2001/XMLSchema#boolean">true</owl:deprecated>
    </owl:Class>
    


    <!-- http://purl.obolibrary.org/obo/FOODON_03411779 -->

    <owl:Class rdf:about="http://purl.obolibrary.org/obo/FOODON_03411779">
        <rdfs:subClassOf rdf:resource="http://www.geneontology.org/formats/oboInOwl#ObsoleteClass"/>
        <obo:IAO_0000231 xml:lang="en">Duplicate entry of *YELLOWTAIL [B1779]*.
&lt;SCISYN&gt;Seriola dorsalis (Gill, 1863)</obo:IAO_0000231>
        <obo:IAO_0000412>http://langual.org</obo:IAO_0000412>
        <obo:IAO_0100001 rdf:datatype="http://www.w3.org/2001/XMLSchema#anyURI">http://purl.obolibrary.org/obo/FOODON_03411534</obo:IAO_0100001>
        <oboInOwl:hasDbXref>LANGUAL:B1779</oboInOwl:hasDbXref>
        <rdfs:comment xml:lang="en">LanguaL curation note: This term is only kept for backward compatibility. DO NOT USE for new indexing.</rdfs:comment>
        <rdfs:label xml:lang="en">california yellowtail (deprecated)</rdfs:label>
        <owl:deprecated rdf:datatype="http://www.w3.org/2001/XMLSchema#boolean">true</owl:deprecated>
    </owl:Class>
    


    <!-- http://purl.obolibrary.org/obo/FOODON_03411847 -->

    <owl:Class rdf:about="http://purl.obolibrary.org/obo/FOODON_03411847">
        <rdfs:subClassOf rdf:resource="http://www.geneontology.org/formats/oboInOwl#ObsoleteClass"/>
        <obo:IAO_0000115 xml:lang="en">Synonym of *CHILEAN PILCHARD [B1847]*</obo:IAO_0000115>
        <obo:IAO_0000412>http://langual.org</obo:IAO_0000412>
        <oboInOwl:hasDbXref>LANGUAL:B1847</oboInOwl:hasDbXref>
        <rdfs:comment xml:lang="en">LanguaL curation note: This term is only kept for backward compatibility. DO NOT USE for new indexing.</rdfs:comment>
        <rdfs:label xml:lang="en">pacific sardine (deprecated)</rdfs:label>
        <owl:deprecated rdf:datatype="http://www.w3.org/2001/XMLSchema#boolean">true</owl:deprecated>
    </owl:Class>
    


    <!-- http://purl.obolibrary.org/obo/FOODON_03411953 -->

    <owl:Class rdf:about="http://purl.obolibrary.org/obo/FOODON_03411953">
        <rdfs:subClassOf rdf:resource="http://www.geneontology.org/formats/oboInOwl#ObsoleteClass"/>
        <obo:IAO_0000231 xml:lang="en">Descriptor inactivated due to duplication.</obo:IAO_0000231>
        <obo:IAO_0000412>http://langual.org</obo:IAO_0000412>
        <oboInOwl:hasDbXref>LANGUAL:B1953</oboInOwl:hasDbXref>
        <rdfs:comment xml:lang="en">LanguaL curation note: This term is only kept for backward compatibility. DO NOT USE for new indexing.</rdfs:comment>
        <rdfs:label xml:lang="en">ocean quahog (deprecated)</rdfs:label>
        <owl:deprecated rdf:datatype="http://www.w3.org/2001/XMLSchema#boolean">true</owl:deprecated>
    </owl:Class>
    


    <!-- http://purl.obolibrary.org/obo/FOODON_03412101 -->

    <owl:Class rdf:about="http://purl.obolibrary.org/obo/FOODON_03412101">
        <rdfs:subClassOf rdf:resource="http://www.geneontology.org/formats/oboInOwl#ObsoleteClass"/>
        <obo:IAO_0000412>http://langual.org</obo:IAO_0000412>
        <oboInOwl:hasDbXref>LANGUAL:B2101</oboInOwl:hasDbXref>
        <rdfs:label xml:lang="en">sheep and goat (deprecated)</rdfs:label>
        <owl:deprecated rdf:datatype="http://www.w3.org/2001/XMLSchema#boolean">true</owl:deprecated>
    </owl:Class>
    


    <!-- http://purl.obolibrary.org/obo/FOODON_03412201 -->

    <owl:Class rdf:about="http://purl.obolibrary.org/obo/FOODON_03412201">
        <rdfs:subClassOf rdf:resource="http://www.geneontology.org/formats/oboInOwl#ObsoleteClass"/>
        <obo:IAO_0000115 xml:lang="en">Descriptor inactivated.</obo:IAO_0000115>
        <obo:IAO_0000412>http://langual.org</obo:IAO_0000412>
        <oboInOwl:hasDbXref>LANGUAL:B2201</oboInOwl:hasDbXref>
        <rdfs:comment xml:lang="en">LanguaL curation note: This term is only kept for backward compatibility. DO NOT USE for new indexing.</rdfs:comment>
        <rdfs:label xml:lang="en">panulirus rissore (deprecated)</rdfs:label>
        <owl:deprecated rdf:datatype="http://www.w3.org/2001/XMLSchema#boolean">true</owl:deprecated>
    </owl:Class>
    


    <!-- http://purl.obolibrary.org/obo/FOODON_03412242 -->

    <owl:Class rdf:about="http://purl.obolibrary.org/obo/FOODON_03412242">
        <rdfs:subClassOf rdf:resource="http://www.geneontology.org/formats/oboInOwl#ObsoleteClass"/>
        <obo:IAO_0000412>http://langual.org</obo:IAO_0000412>
        <oboInOwl:hasDbXref>LANGUAL:B2242</oboInOwl:hasDbXref>
        <rdfs:label xml:lang="en">swine and calf (deprecated)</rdfs:label>
        <owl:deprecated rdf:datatype="http://www.w3.org/2001/XMLSchema#boolean">true</owl:deprecated>
    </owl:Class>
    


    <!-- http://purl.obolibrary.org/obo/FOODON_03412243 -->

    <owl:Class rdf:about="http://purl.obolibrary.org/obo/FOODON_03412243">
        <rdfs:subClassOf rdf:resource="http://www.geneontology.org/formats/oboInOwl#ObsoleteClass"/>
        <obo:IAO_0000412>http://langual.org</obo:IAO_0000412>
        <oboInOwl:hasDbXref>LANGUAL:B2243</oboInOwl:hasDbXref>
        <rdfs:label xml:lang="en">cattle and swine and sheep (deprecated)</rdfs:label>
        <owl:deprecated rdf:datatype="http://www.w3.org/2001/XMLSchema#boolean">true</owl:deprecated>
    </owl:Class>
    


    <!-- http://purl.obolibrary.org/obo/FOODON_03412244 -->

    <owl:Class rdf:about="http://purl.obolibrary.org/obo/FOODON_03412244">
        <rdfs:subClassOf rdf:resource="http://www.geneontology.org/formats/oboInOwl#ObsoleteClass"/>
        <obo:IAO_0000412>http://langual.org</obo:IAO_0000412>
        <oboInOwl:hasDbXref>LANGUAL:B2244</oboInOwl:hasDbXref>
        <rdfs:label xml:lang="en">cattle and sheep (deprecated)</rdfs:label>
        <owl:deprecated rdf:datatype="http://www.w3.org/2001/XMLSchema#boolean">true</owl:deprecated>
    </owl:Class>
    


    <!-- http://purl.obolibrary.org/obo/FOODON_03412245 -->

    <owl:Class rdf:about="http://purl.obolibrary.org/obo/FOODON_03412245">
        <rdfs:subClassOf rdf:resource="http://www.geneontology.org/formats/oboInOwl#ObsoleteClass"/>
        <obo:IAO_0000412>http://langual.org</obo:IAO_0000412>
        <oboInOwl:hasDbXref>LANGUAL:B2245</oboInOwl:hasDbXref>
        <rdfs:label xml:lang="en">cattle and goat (deprecated)</rdfs:label>
        <owl:deprecated rdf:datatype="http://www.w3.org/2001/XMLSchema#boolean">true</owl:deprecated>
    </owl:Class>
    


    <!-- http://purl.obolibrary.org/obo/FOODON_03412247 -->

    <owl:Class rdf:about="http://purl.obolibrary.org/obo/FOODON_03412247">
        <rdfs:subClassOf rdf:resource="http://www.geneontology.org/formats/oboInOwl#ObsoleteClass"/>
        <obo:IAO_0000412>http://langual.org</obo:IAO_0000412>
        <oboInOwl:hasDbXref>LANGUAL:B2247</oboInOwl:hasDbXref>
        <rdfs:label xml:lang="en">cattle and sheep and goat (deprecated)</rdfs:label>
        <owl:deprecated rdf:datatype="http://www.w3.org/2001/XMLSchema#boolean">true</owl:deprecated>
    </owl:Class>
    


    <!-- http://purl.obolibrary.org/obo/FOODON_03412282 -->

    <owl:Class rdf:about="http://purl.obolibrary.org/obo/FOODON_03412282">
        <rdfs:subClassOf rdf:resource="http://www.geneontology.org/formats/oboInOwl#ObsoleteClass"/>
        <obo:IAO_0000115 xml:lang="en">School shark is a synonym of TOPE SHARK [B2525], which should be used instead.</obo:IAO_0000115>
        <obo:IAO_0000412>http://langual.org</obo:IAO_0000412>
        <oboInOwl:hasDbXref>LANGUAL:B2282</oboInOwl:hasDbXref>
        <rdfs:comment xml:lang="en">LanguaL curation note: This term is only kept for backward compatibility. DO NOT USE for new indexing.</rdfs:comment>
        <rdfs:label xml:lang="en">school shark (deprecated)</rdfs:label>
        <owl:deprecated rdf:datatype="http://www.w3.org/2001/XMLSchema#boolean">true</owl:deprecated>
    </owl:Class>
    


    <!-- http://purl.obolibrary.org/obo/FOODON_03412379 -->

    <owl:Class rdf:about="http://purl.obolibrary.org/obo/FOODON_03412379">
        <rdfs:subClassOf rdf:resource="http://www.geneontology.org/formats/oboInOwl#ObsoleteClass"/>
        <obo:IAO_0000412>http://langual.org</obo:IAO_0000412>
        <oboInOwl:hasDbXref>LANGUAL:B2379</oboInOwl:hasDbXref>
        <rdfs:comment xml:lang="en">LanguaL curation note: This term is only kept for backward compatibility. DO NOT USE for new indexing.</rdfs:comment>
        <rdfs:label xml:lang="en">carmine cusk-eel (deprecated)</rdfs:label>
        <owl:deprecated rdf:datatype="http://www.w3.org/2001/XMLSchema#boolean">true</owl:deprecated>
    </owl:Class>
    


    <!-- http://purl.obolibrary.org/obo/FOODON_03412381 -->

    <owl:Class rdf:about="http://purl.obolibrary.org/obo/FOODON_03412381">
        <rdfs:subClassOf rdf:resource="http://www.geneontology.org/formats/oboInOwl#ObsoleteClass"/>
        <obo:IAO_0000115 xml:lang="en">Species unknown.</obo:IAO_0000115>
        <obo:IAO_0000412>http://langual.org</obo:IAO_0000412>
        <oboInOwl:hasDbXref>LANGUAL:B2381</oboInOwl:hasDbXref>
        <rdfs:comment xml:lang="en">LanguaL curation note: This term is only kept for backward compatibility. DO NOT USE for new indexing.</rdfs:comment>
        <rdfs:label xml:lang="en">lutjanus silla (deprecated)</rdfs:label>
        <owl:deprecated rdf:datatype="http://www.w3.org/2001/XMLSchema#boolean">true</owl:deprecated>
    </owl:Class>
    


    <!-- http://purl.obolibrary.org/obo/FOODON_03412387 -->

    <owl:Class rdf:about="http://purl.obolibrary.org/obo/FOODON_03412387">
        <rdfs:subClassOf rdf:resource="http://www.geneontology.org/formats/oboInOwl#ObsoleteClass"/>
        <obo:IAO_0000115 xml:lang="en">Synonym of *PIKE PERCH [B1399]*</obo:IAO_0000115>
        <obo:IAO_0000412>http://langual.org</obo:IAO_0000412>
        <oboInOwl:hasDbXref>LANGUAL:B2387</oboInOwl:hasDbXref>
        <rdfs:comment xml:lang="en">LanguaL curation note: This term is only kept for backward compatibility. DO NOT USE for new indexing.</rdfs:comment>
        <rdfs:label xml:lang="en">zander (deprecated)</rdfs:label>
        <owl:deprecated rdf:datatype="http://www.w3.org/2001/XMLSchema#boolean">true</owl:deprecated>
    </owl:Class>
    


    <!-- http://purl.obolibrary.org/obo/FOODON_03412396 -->

    <owl:Class rdf:about="http://purl.obolibrary.org/obo/FOODON_03412396">
        <rdfs:subClassOf rdf:resource="http://www.geneontology.org/formats/oboInOwl#ObsoleteClass"/>
        <obo:IAO_0000412>http://langual.org</obo:IAO_0000412>
        <oboInOwl:hasDbXref>LANGUAL:B2396</oboInOwl:hasDbXref>
        <rdfs:label xml:lang="en">cattle and lamb (deprecated)</rdfs:label>
        <owl:deprecated rdf:datatype="http://www.w3.org/2001/XMLSchema#boolean">true</owl:deprecated>
    </owl:Class>
    


    <!-- http://purl.obolibrary.org/obo/FOODON_03412466 -->

    <owl:Class rdf:about="http://purl.obolibrary.org/obo/FOODON_03412466">
        <rdfs:subClassOf rdf:resource="http://www.geneontology.org/formats/oboInOwl#ObsoleteClass"/>
        <obo:IAO_0000412>http://langual.org</obo:IAO_0000412>
        <oboInOwl:hasDbXref>LANGUAL:B2466</oboInOwl:hasDbXref>
        <rdfs:comment xml:lang="en">LanguaL curation note: This term is only kept for backward compatibility. DO NOT USE for new indexing.</rdfs:comment>
        <rdfs:label xml:lang="en">snow pea (deprecated)</rdfs:label>
        <owl:deprecated rdf:datatype="http://www.w3.org/2001/XMLSchema#boolean">true</owl:deprecated>
    </owl:Class>
    


    <!-- http://purl.obolibrary.org/obo/FOODON_03412467 -->

    <owl:Class rdf:about="http://purl.obolibrary.org/obo/FOODON_03412467">
        <rdfs:subClassOf rdf:resource="http://www.geneontology.org/formats/oboInOwl#ObsoleteClass"/>
        <obo:IAO_0000412>http://langual.org</obo:IAO_0000412>
        <oboInOwl:hasDbXref>LANGUAL:B2467</oboInOwl:hasDbXref>
        <rdfs:comment xml:lang="en">LanguaL curation note: This term is only kept for backward compatibility. DO NOT USE for new indexing.</rdfs:comment>
        <rdfs:label xml:lang="en">sugar pea, edible pod (deprecated)</rdfs:label>
        <owl:deprecated rdf:datatype="http://www.w3.org/2001/XMLSchema#boolean">true</owl:deprecated>
    </owl:Class>
    


    <!-- http://purl.obolibrary.org/obo/FOODON_03412664 -->

    <owl:Class rdf:about="http://purl.obolibrary.org/obo/FOODON_03412664">
        <rdfs:subClassOf rdf:resource="http://www.geneontology.org/formats/oboInOwl#ObsoleteClass"/>
        <obo:IAO_0000412>http://langual.org</obo:IAO_0000412>
        <obo:IAO_0100001 rdf:resource="http://purl.obolibrary.org/obo/FOODON_03411814"/>
        <oboInOwl:hasDbXref>LANGUAL:B2664</oboInOwl:hasDbXref>
        <rdfs:comment xml:lang="en">LanguaL curation note: This term is only kept for backward compatibility. DO NOT USE for new indexing.</rdfs:comment>
        <rdfs:label xml:lang="en">corvina (deprecated)</rdfs:label>
        <owl:deprecated rdf:datatype="http://www.w3.org/2001/XMLSchema#boolean">true</owl:deprecated>
    </owl:Class>
    


    <!-- http://purl.obolibrary.org/obo/FOODON_03412700 -->

    <owl:Class rdf:about="http://purl.obolibrary.org/obo/FOODON_03412700">
        <rdfs:subClassOf rdf:resource="http://www.geneontology.org/formats/oboInOwl#ObsoleteClass"/>
        <obo:IAO_0000115 xml:lang="en">FDA market name for Amercan eel, Anguilla rostrata (Lesueur, 1817).</obo:IAO_0000115>
        <obo:IAO_0000412>http://langual.org</obo:IAO_0000412>
        <oboInOwl:hasDbXref>LANGUAL:B2700</oboInOwl:hasDbXref>
        <rdfs:comment xml:lang="en">LanguaL curation note: This term is only kept for backward compatibility. DO NOT USE for new indexing.</rdfs:comment>
        <rdfs:label xml:lang="en">eel, freshwater (deprecated)</rdfs:label>
        <owl:deprecated rdf:datatype="http://www.w3.org/2001/XMLSchema#boolean">true</owl:deprecated>
    </owl:Class>
    


    <!-- http://purl.obolibrary.org/obo/FOODON_03412826 -->

    <owl:Class rdf:about="http://purl.obolibrary.org/obo/FOODON_03412826">
        <rdfs:subClassOf rdf:resource="http://www.geneontology.org/formats/oboInOwl#ObsoleteClass"/>
        <obo:IAO_0000115 xml:lang="en">Species unknown.</obo:IAO_0000115>
        <obo:IAO_0000412>http://langual.org</obo:IAO_0000412>
        <oboInOwl:hasDbXref>LANGUAL:B2826</oboInOwl:hasDbXref>
        <rdfs:comment xml:lang="en">LanguaL curation note: This term is only kept for backward compatibility. DO NOT USE for new indexing.</rdfs:comment>
        <rdfs:label xml:lang="en">belwisia (deprecated)</rdfs:label>
        <owl:deprecated rdf:datatype="http://www.w3.org/2001/XMLSchema#boolean">true</owl:deprecated>
    </owl:Class>
    


    <!-- http://purl.obolibrary.org/obo/FOODON_03413066 -->

    <owl:Class rdf:about="http://purl.obolibrary.org/obo/FOODON_03413066">
        <rdfs:subClassOf rdf:resource="http://www.geneontology.org/formats/oboInOwl#ObsoleteClass"/>
        <obo:IAO_0000119>If used for food additives, this descriptor refers to the European Commission food additive regulation according to the four Food Additive Directives: the EEC Framework Directive on Food Additives (89/107/EEC), the Directive on colours (94/36/EC), the Directive on sweeteners (94/35/EC) and the &apos;miscellaneous&apos; Directive (95/2/EC) [http://ec.europa.eu/food/fs/sfp/flav_index_en.html] and/or Codex Alimentarius Commission General Standard for Food Additives (CODEX STAN 192) [http://www.codexalimentarius.net/download/standards/4/CXS_192e.pdf].

If used for food supplement substances, this descriptor refers to the European Commission regulation in general [http://ec.europa.eu/food/food/labellingnutrition/supplements/index_en.htm] and specifically to the EC Directive on the approximation of the laws of the Members States relating to food supplements (2002/46/EC) [http://eur-lex.europa.eu/LexUriServ/LexUriServ.do?uri=OJ:L:2002:183:0051:0057:EN:PDF].</obo:IAO_0000119>
        <obo:IAO_0000412>http://langual.org</obo:IAO_0000412>
        <oboInOwl:hasDbXref>LANGUAL:B3066</oboInOwl:hasDbXref>
        <rdfs:comment xml:lang="en">LanguaL curation note: This term is only kept for backward compatibility. DO NOT USE for new indexing.</rdfs:comment>
        <rdfs:label xml:lang="en">citric acid (deprecated)</rdfs:label>
        <owl:deprecated rdf:datatype="http://www.w3.org/2001/XMLSchema#boolean">true</owl:deprecated>
    </owl:Class>
    


    <!-- http://purl.obolibrary.org/obo/FOODON_03413165 -->

    <owl:Class rdf:about="http://purl.obolibrary.org/obo/FOODON_03413165">
        <rdfs:subClassOf rdf:resource="http://www.geneontology.org/formats/oboInOwl#ObsoleteClass"/>
        <obo:IAO_0000412>http://langual.org</obo:IAO_0000412>
        <oboInOwl:hasDbXref>LANGUAL:B3165</oboInOwl:hasDbXref>
        <rdfs:comment xml:lang="en">LanguaL curation note: This term is only kept for backward compatibility. DO NOT USE for new indexing.</rdfs:comment>
        <rdfs:label xml:lang="en">monosodium glutamate (deprecated)</rdfs:label>
        <owl:deprecated rdf:datatype="http://www.w3.org/2001/XMLSchema#boolean">true</owl:deprecated>
    </owl:Class>
    


    <!-- http://purl.obolibrary.org/obo/FOODON_03413206 -->

    <owl:Class rdf:about="http://purl.obolibrary.org/obo/FOODON_03413206">
        <rdfs:subClassOf rdf:resource="http://www.geneontology.org/formats/oboInOwl#ObsoleteClass"/>
        <obo:IAO_0000412>http://langual.org</obo:IAO_0000412>
        <oboInOwl:hasDbXref>LANGUAL:B3206</oboInOwl:hasDbXref>
        <rdfs:comment xml:lang="en">LanguaL curation note: This term is only kept for backward compatibility. DO NOT USE for new indexing.</rdfs:comment>
        <rdfs:label xml:lang="en">potassium chloride (deprecated)</rdfs:label>
        <owl:deprecated rdf:datatype="http://www.w3.org/2001/XMLSchema#boolean">true</owl:deprecated>
    </owl:Class>
    


    <!-- http://purl.obolibrary.org/obo/FOODON_03413256 -->

    <owl:Class rdf:about="http://purl.obolibrary.org/obo/FOODON_03413256">
        <rdfs:subClassOf rdf:resource="http://www.geneontology.org/formats/oboInOwl#ObsoleteClass"/>
        <obo:IAO_0000412>http://langual.org</obo:IAO_0000412>
        <oboInOwl:hasDbXref>LANGUAL:B3256</oboInOwl:hasDbXref>
        <rdfs:comment xml:lang="en">LanguaL curation note: This term is only kept for backward compatibility. DO NOT USE for new indexing.</rdfs:comment>
        <rdfs:label xml:lang="en">sodium hydrogen carbonate (deprecated)</rdfs:label>
        <owl:deprecated rdf:datatype="http://www.w3.org/2001/XMLSchema#boolean">true</owl:deprecated>
    </owl:Class>
    


    <!-- http://purl.obolibrary.org/obo/FOODON_03413412 -->

    <owl:Class rdf:about="http://purl.obolibrary.org/obo/FOODON_03413412">
        <rdfs:subClassOf rdf:resource="http://www.geneontology.org/formats/oboInOwl#ObsoleteClass"/>
        <obo:IAO_0000412>http://langual.org</obo:IAO_0000412>
        <oboInOwl:hasDbXref>LANGUAL:B3412</oboInOwl:hasDbXref>
        <rdfs:comment xml:lang="en">LanguaL curation note: This term is only kept for backward compatibility. DO NOT USE for new indexing.</rdfs:comment>
        <rdfs:label xml:lang="en">japanese-green (deprecated)</rdfs:label>
        <owl:deprecated rdf:datatype="http://www.w3.org/2001/XMLSchema#boolean">true</owl:deprecated>
    </owl:Class>
    


    <!-- http://purl.obolibrary.org/obo/FOODON_03414301 -->

    <owl:Class rdf:about="http://purl.obolibrary.org/obo/FOODON_03414301">
        <rdfs:subClassOf rdf:resource="http://www.geneontology.org/formats/oboInOwl#ObsoleteClass"/>
        <obo:IAO_0000412>http://langual.org</obo:IAO_0000412>
        <oboInOwl:hasDbXref>LANGUAL:B4301</oboInOwl:hasDbXref>
        <rdfs:label xml:lang="en">mustard and cress (deprecated)</rdfs:label>
        <owl:deprecated rdf:datatype="http://www.w3.org/2001/XMLSchema#boolean">true</owl:deprecated>
    </owl:Class>
    


    <!-- http://purl.obolibrary.org/obo/FOODON_03414352 -->

    <owl:Class rdf:about="http://purl.obolibrary.org/obo/FOODON_03414352">
        <rdfs:subClassOf rdf:resource="http://www.geneontology.org/formats/oboInOwl#ObsoleteClass"/>
        <obo:IAO_0000119>WIKIPEDIA:Aframomum_melegueta</obo:IAO_0000119>
        <obo:IAO_0000231 xml:lang="en">Descriptor inactivated due to duplication.</obo:IAO_0000231>
        <obo:IAO_0000412>http://langual.org</obo:IAO_0000412>
        <oboInOwl:hasDbXref>LANGUAL:B4352</oboInOwl:hasDbXref>
        <rdfs:comment xml:lang="en">LanguaL curation note: This term is only kept for backward compatibility. DO NOT USE for new indexing.</rdfs:comment>
        <rdfs:label xml:lang="en">grains-of-paradise (deprecated)</rdfs:label>
        <owl:deprecated rdf:datatype="http://www.w3.org/2001/XMLSchema#boolean">true</owl:deprecated>
    </owl:Class>
    


    <!-- http://purl.obolibrary.org/obo/FOODON_03420001 -->

    <owl:Class rdf:about="http://purl.obolibrary.org/obo/FOODON_03420001">
        <rdfs:subClassOf rdf:resource="http://www.geneontology.org/formats/oboInOwl#ObsoleteClass"/>
        <obo:IAO_0000412>http://langual.org</obo:IAO_0000412>
        <oboInOwl:hasDbXref>LANGUAL:C0001</oboInOwl:hasDbXref>
        <rdfs:comment xml:lang="en">LanguaL curation note: Used only in conjunction with *FOOD SOURCE NOT KNOWN*, i.e., if it is not known whether the food source is animal, plant, microorganism or chemical.</rdfs:comment>
        <rdfs:label xml:lang="en">part of plant or animal not known (deprecated)</rdfs:label>
        <owl:deprecated rdf:datatype="http://www.w3.org/2001/XMLSchema#boolean">true</owl:deprecated>
    </owl:Class>
    


    <!-- http://purl.obolibrary.org/obo/FOODON_03420005 -->

    <owl:Class rdf:about="http://purl.obolibrary.org/obo/FOODON_03420005">
        <rdfs:subClassOf rdf:resource="http://www.geneontology.org/formats/oboInOwl#ObsoleteClass"/>
        <obo:IAO_0000412>http://langual.org</obo:IAO_0000412>
        <oboInOwl:hasDbXref>LANGUAL:C0005</oboInOwl:hasDbXref>
        <rdfs:comment xml:lang="en">LanguaL curation note: Used only for chemical food products.</rdfs:comment>
        <rdfs:label xml:lang="en">part of plant or animal not applicable (deprecated)</rdfs:label>
        <owl:deprecated rdf:datatype="http://www.w3.org/2001/XMLSchema#boolean">true</owl:deprecated>
    </owl:Class>
    


    <!-- http://purl.obolibrary.org/obo/FOODON_03420246 -->

    <owl:Class rdf:about="http://purl.obolibrary.org/obo/FOODON_03420246">
        <rdfs:subClassOf rdf:resource="http://www.geneontology.org/formats/oboInOwl#ObsoleteClass"/>
        <obo:IAO_0000412>http://langual.org</obo:IAO_0000412>
        <oboInOwl:hasDbXref>LANGUAL:C0246</oboInOwl:hasDbXref>
        <rdfs:label xml:lang="en">ink, aquatic animal (deprecated)</rdfs:label>
        <owl:deprecated rdf:datatype="http://www.w3.org/2001/XMLSchema#boolean">true</owl:deprecated>
    </owl:Class>
    


    <!-- http://purl.obolibrary.org/obo/FOODON_03430001 -->

    <owl:Class rdf:about="http://purl.obolibrary.org/obo/FOODON_03430001">
        <rdfs:subClassOf rdf:resource="http://www.geneontology.org/formats/oboInOwl#ObsoleteClass"/>
        <obo:IAO_0000412>http://langual.org</obo:IAO_0000412>
        <oboInOwl:hasDbXref>LANGUAL:E0001</oboInOwl:hasDbXref>
        <rdfs:comment xml:lang="en">LanguaL curation note: Used when nothing is known about the physical state, shape or form of the food product.</rdfs:comment>
        <rdfs:label xml:lang="en">physical state, shape or form not known (deprecated)</rdfs:label>
        <owl:deprecated rdf:datatype="http://www.w3.org/2001/XMLSchema#boolean">true</owl:deprecated>
    </owl:Class>
    


    <!-- http://purl.obolibrary.org/obo/FOODON_03430172 -->

    <owl:Class rdf:about="http://purl.obolibrary.org/obo/FOODON_03430172">
        <rdfs:subClassOf rdf:resource="http://www.geneontology.org/formats/oboInOwl#ObsoleteClass"/>
        <obo:IAO_0000115 xml:lang="en">Other liquid or powder forms for ingestion in dose amounts. Other forms not represented for use as a conventional food or as a sole item of a meal or the diet.</obo:IAO_0000115>
        <obo:IAO_0000412>http://langual.org</obo:IAO_0000412>
        <oboInOwl:hasDbXref>LANGUAL:E0172</oboInOwl:hasDbXref>
        <rdfs:label xml:lang="en">supplement form, other (deprecated)</rdfs:label>
        <owl:deprecated rdf:datatype="http://www.w3.org/2001/XMLSchema#boolean">true</owl:deprecated>
    </owl:Class>
    


    <!-- http://purl.obolibrary.org/obo/FOODON_03430177 -->

    <owl:Class rdf:about="http://purl.obolibrary.org/obo/FOODON_03430177">
        <rdfs:subClassOf rdf:resource="http://www.geneontology.org/formats/oboInOwl#ObsoleteClass"/>
        <obo:IAO_0000412>http://langual.org</obo:IAO_0000412>
        <oboInOwl:hasDbXref>LANGUAL:E0177</oboInOwl:hasDbXref>
        <rdfs:comment xml:lang="en">LanguaL curation note: Used when nothing is known about the form of the dietary supplement.</rdfs:comment>
        <rdfs:label xml:lang="en">supplement form, unknown (deprecated)</rdfs:label>
        <owl:deprecated rdf:datatype="http://www.w3.org/2001/XMLSchema#boolean">true</owl:deprecated>
    </owl:Class>
    


    <!-- http://purl.obolibrary.org/obo/FOODON_03440001 -->

    <owl:Class rdf:about="http://purl.obolibrary.org/obo/FOODON_03440001">
        <rdfs:subClassOf rdf:resource="http://www.geneontology.org/formats/oboInOwl#ObsoleteClass"/>
        <obo:IAO_0000412>http://langual.org</obo:IAO_0000412>
        <oboInOwl:hasDbXref>LANGUAL:F0001</oboInOwl:hasDbXref>
        <rdfs:comment xml:lang="en">LanguaL curation note: Used only when no information is available about the use of or degree of heat treatment performed.</rdfs:comment>
        <rdfs:label xml:lang="en">extent of heat treatment not known (deprecated)</rdfs:label>
        <owl:deprecated rdf:datatype="http://www.w3.org/2001/XMLSchema#boolean">true</owl:deprecated>
    </owl:Class>
    


    <!-- http://purl.obolibrary.org/obo/FOODON_03480001 -->

    <owl:Class rdf:about="http://purl.obolibrary.org/obo/FOODON_03480001">
        <rdfs:subClassOf rdf:resource="http://www.geneontology.org/formats/oboInOwl#ObsoleteClass"/>
        <obo:IAO_0000412>http://langual.org</obo:IAO_0000412>
        <oboInOwl:hasDbXref>LANGUAL:K0001</oboInOwl:hasDbXref>
        <rdfs:comment xml:lang="en">LanguaL curation note: Used when nothing is known about the packing medium, if any is present.</rdfs:comment>
        <rdfs:label xml:lang="en">packing medium not known (deprecated)</rdfs:label>
        <owl:deprecated rdf:datatype="http://www.w3.org/2001/XMLSchema#boolean">true</owl:deprecated>
    </owl:Class>
    


    <!-- http://purl.obolibrary.org/obo/FOODON_03480004 -->

    <owl:Class rdf:about="http://purl.obolibrary.org/obo/FOODON_03480004">
        <rdfs:subClassOf rdf:resource="http://www.geneontology.org/formats/oboInOwl#ObsoleteClass"/>
        <obo:IAO_0000412>http://langual.org</obo:IAO_0000412>
        <oboInOwl:hasDbXref>LANGUAL:K0004</oboInOwl:hasDbXref>
        <rdfs:comment xml:lang="en">LanguaL curation note: Used when the packing medium does not fall under any of the major categories listed.</rdfs:comment>
        <rdfs:label xml:lang="en">packing medium, other (deprecated)</rdfs:label>
        <owl:deprecated rdf:datatype="http://www.w3.org/2001/XMLSchema#boolean">true</owl:deprecated>
    </owl:Class>
    


    <!-- http://purl.obolibrary.org/obo/FOODON_03490001 -->

    <owl:Class rdf:about="http://purl.obolibrary.org/obo/FOODON_03490001">
        <rdfs:subClassOf rdf:resource="http://www.geneontology.org/formats/oboInOwl#ObsoleteClass"/>
        <obo:IAO_0000412>http://langual.org</obo:IAO_0000412>
        <oboInOwl:hasDbXref>LANGUAL:M0001</oboInOwl:hasDbXref>
        <rdfs:comment xml:lang="en">LanguaL curation note: Used when it is not known what container or wrapping, if any, is present.</rdfs:comment>
        <rdfs:label xml:lang="en">container or wrapping not known (deprecated)</rdfs:label>
        <owl:deprecated rdf:datatype="http://www.w3.org/2001/XMLSchema#boolean">true</owl:deprecated>
    </owl:Class>
    


    <!-- http://purl.obolibrary.org/obo/FOODON_03490003 -->

    <owl:Class rdf:about="http://purl.obolibrary.org/obo/FOODON_03490003">
        <rdfs:subClassOf rdf:resource="http://www.geneontology.org/formats/oboInOwl#ObsoleteClass"/>
        <obo:IAO_0000412>http://langual.org</obo:IAO_0000412>
        <oboInOwl:hasDbXref>LANGUAL:M0003</oboInOwl:hasDbXref>
        <rdfs:comment xml:lang="en">LanguaL curation note: Used when the food product is not packaged in a container or wrapping. includes products that are coated with a thin layer of wax, e.g., fruits or vegetables, but are not further packaged.</rdfs:comment>
        <rdfs:label xml:lang="en">no container or wrapping used (deprecated)</rdfs:label>
        <owl:deprecated rdf:datatype="http://www.w3.org/2001/XMLSchema#boolean">true</owl:deprecated>
    </owl:Class>
    


    <!-- http://purl.obolibrary.org/obo/FOODON_03490004 -->

    <owl:Class rdf:about="http://purl.obolibrary.org/obo/FOODON_03490004">
        <rdfs:subClassOf rdf:resource="http://www.geneontology.org/formats/oboInOwl#ObsoleteClass"/>
        <obo:IAO_0000412>http://langual.org</obo:IAO_0000412>
        <oboInOwl:hasDbXref>LANGUAL:M0004</oboInOwl:hasDbXref>
        <rdfs:comment xml:lang="en">LanguaL curation note: Used when the container does not fall under any of the major types listed.</rdfs:comment>
        <rdfs:label xml:lang="en">container or wrapping, other (deprecated)</rdfs:label>
        <owl:deprecated rdf:datatype="http://www.w3.org/2001/XMLSchema#boolean">true</owl:deprecated>
    </owl:Class>
    


    <!-- http://purl.obolibrary.org/obo/FOODON_03500001 -->

    <owl:Class rdf:about="http://purl.obolibrary.org/obo/FOODON_03500001">
        <rdfs:subClassOf rdf:resource="http://www.geneontology.org/formats/oboInOwl#ObsoleteClass"/>
        <obo:IAO_0000412>http://langual.org</obo:IAO_0000412>
        <oboInOwl:hasDbXref>LANGUAL:N0001</oboInOwl:hasDbXref>
        <rdfs:comment xml:lang="en">LanguaL curation note: Used when it is not known what the food contact surface is, if any.</rdfs:comment>
        <rdfs:label xml:lang="en">food contact surface not known (deprecated)</rdfs:label>
        <owl:deprecated rdf:datatype="http://www.w3.org/2001/XMLSchema#boolean">true</owl:deprecated>
    </owl:Class>
    


    <!-- http://purl.obolibrary.org/obo/FOODON_03500003 -->

    <owl:Class rdf:about="http://purl.obolibrary.org/obo/FOODON_03500003">
        <rdfs:subClassOf rdf:resource="http://www.geneontology.org/formats/oboInOwl#ObsoleteClass"/>
        <obo:IAO_0000412>http://langual.org</obo:IAO_0000412>
        <oboInOwl:hasDbXref>LANGUAL:N0003</oboInOwl:hasDbXref>
        <rdfs:comment xml:lang="en">LanguaL curation note: Used when the product is neither packed nor coated with a protective coating.</rdfs:comment>
        <rdfs:label xml:lang="en">no food contact surface present (deprecated)</rdfs:label>
        <owl:deprecated rdf:datatype="http://www.w3.org/2001/XMLSchema#boolean">true</owl:deprecated>
    </owl:Class>
    


    <!-- http://purl.obolibrary.org/obo/FOODON_03500004 -->

    <owl:Class rdf:about="http://purl.obolibrary.org/obo/FOODON_03500004">
        <rdfs:subClassOf rdf:resource="http://www.geneontology.org/formats/oboInOwl#ObsoleteClass"/>
        <obo:IAO_0000412>http://langual.org</obo:IAO_0000412>
        <oboInOwl:hasDbXref>LANGUAL:N0004</oboInOwl:hasDbXref>
        <rdfs:comment xml:lang="en">LanguaL curation note: Used only if the contact surface does not fall under any of the major types listed.</rdfs:comment>
        <rdfs:label xml:lang="en">food contact surface, other (deprecated)</rdfs:label>
        <owl:deprecated rdf:datatype="http://www.w3.org/2001/XMLSchema#boolean">true</owl:deprecated>
    </owl:Class>
    


    <!-- http://purl.obolibrary.org/obo/FOODON_03510001 -->

    <owl:Class rdf:about="http://purl.obolibrary.org/obo/FOODON_03510001">
        <rdfs:subClassOf rdf:resource="http://www.geneontology.org/formats/oboInOwl#ObsoleteClass"/>
        <obo:IAO_0000412>http://langual.org</obo:IAO_0000412>
        <oboInOwl:hasDbXref>LANGUAL:P0001</oboInOwl:hasDbXref>
        <rdfs:comment xml:lang="en">LanguaL curation note: Used when nothing is know about the consumer group.</rdfs:comment>
        <rdfs:label xml:lang="en">consumer group not known (deprecated)</rdfs:label>
        <owl:deprecated rdf:datatype="http://www.w3.org/2001/XMLSchema#boolean">true</owl:deprecated>
    </owl:Class>
    


    <!-- http://purl.obolibrary.org/obo/FOODON_03510003 -->

    <owl:Class rdf:about="http://purl.obolibrary.org/obo/FOODON_03510003">
        <rdfs:subClassOf rdf:resource="http://www.geneontology.org/formats/oboInOwl#ObsoleteClass"/>
        <obo:IAO_0000412>http://langual.org</obo:IAO_0000412>
        <oboInOwl:hasDbXref>LANGUAL:P0003</oboInOwl:hasDbXref>
        <rdfs:label xml:lang="en">consumer group not applicable (deprecated)</rdfs:label>
        <owl:deprecated rdf:datatype="http://www.w3.org/2001/XMLSchema#boolean">true</owl:deprecated>
    </owl:Class>
    


    <!-- http://purl.obolibrary.org/obo/FOODON_03510024 -->

    <owl:Class rdf:about="http://purl.obolibrary.org/obo/FOODON_03510024">
        <rdfs:subClassOf rdf:resource="http://www.geneontology.org/formats/oboInOwl#ObsoleteClass"/>
        <obo:IAO_0000115 xml:lang="en">Food produced and marketed for human use without any restriction by age.</obo:IAO_0000115>
        <obo:IAO_0000412>http://langual.org</obo:IAO_0000412>
        <obo:IAO_0100001 rdf:resource="http://purl.obolibrary.org/obo/FOODON_03510026"/>
        <oboInOwl:hasDbXref>LANGUAL:P0024</oboInOwl:hasDbXref>
        <rdfs:label xml:lang="en">human consumer, no age specification (deprecated)</rdfs:label>
        <owl:deprecated rdf:datatype="http://www.w3.org/2001/XMLSchema#boolean">true</owl:deprecated>
    </owl:Class>
    


    <!-- http://purl.obolibrary.org/obo/FOODON_03510160 -->

    <owl:Class rdf:about="http://purl.obolibrary.org/obo/FOODON_03510160">
        <rdfs:subClassOf rdf:resource="http://www.geneontology.org/formats/oboInOwl#ObsoleteClass"/>
        <obo:IAO_0000115 xml:lang="en">Use these descriptors when indexing food names for which label or labeling information is available. &apos;Labeling&apos; includes all labels and other written, printed or graphic material that appears on a product&apos;s container or wrapping, as well as any such material accompanying a product.</obo:IAO_0000115>
        <obo:IAO_0000412>http://langual.org</obo:IAO_0000412>
        <oboInOwl:hasDbXref>LANGUAL:P0160</oboInOwl:hasDbXref>
        <rdfs:comment xml:lang="en">LanguaL curation note: This term is only kept for backward compatibility. DO NOT USE for new indexing.</rdfs:comment>
        <rdfs:label xml:lang="en">label or labeling claim (deprecated)</rdfs:label>
        <owl:deprecated rdf:datatype="http://www.w3.org/2001/XMLSchema#boolean">true</owl:deprecated>
    </owl:Class>
    


    <!-- http://purl.obolibrary.org/obo/FOODON_03510163 -->

    <owl:Class rdf:about="http://purl.obolibrary.org/obo/FOODON_03510163">
        <rdfs:subClassOf rdf:resource="http://www.geneontology.org/formats/oboInOwl#ObsoleteClass"/>
        <obo:IAO_0000115 xml:lang="en">Use when the &apos;claim or use&apos; index term is derived from written, printed or graphic material that appears on a product&apos;s container or wrapping but is not a part of the food label.</obo:IAO_0000115>
        <obo:IAO_0000412>http://langual.org</obo:IAO_0000412>
        <oboInOwl:hasDbXref>LANGUAL:P0163</oboInOwl:hasDbXref>
        <rdfs:comment xml:lang="en">LanguaL curation note: This term is only kept for backward compatibility. DO NOT USE for new indexing.</rdfs:comment>
        <rdfs:label xml:lang="en">labeling claim (deprecated)</rdfs:label>
        <owl:deprecated rdf:datatype="http://www.w3.org/2001/XMLSchema#boolean">true</owl:deprecated>
    </owl:Class>
    


    <!-- http://purl.obolibrary.org/obo/FOODON_03510258 -->

    <owl:Class rdf:about="http://purl.obolibrary.org/obo/FOODON_03510258">
        <rdfs:subClassOf rdf:resource="http://www.geneontology.org/formats/oboInOwl#ObsoleteClass"/>
        <obo:IAO_0000412>http://langual.org</obo:IAO_0000412>
        <oboInOwl:hasDbXref>LANGUAL:P0258</oboInOwl:hasDbXref>
        <rdfs:label xml:lang="en">human consumer, other (deprecated)</rdfs:label>
        <owl:deprecated rdf:datatype="http://www.w3.org/2001/XMLSchema#boolean">true</owl:deprecated>
    </owl:Class>
    


    <!-- http://purl.obolibrary.org/obo/FOODON_03520001 -->

    <owl:Class rdf:about="http://purl.obolibrary.org/obo/FOODON_03520001">
        <rdfs:subClassOf rdf:resource="http://www.geneontology.org/formats/oboInOwl#ObsoleteClass"/>
        <obo:IAO_0000412>http://langual.org</obo:IAO_0000412>
        <oboInOwl:hasDbXref>LANGUAL:R0001</oboInOwl:hasDbXref>
        <rdfs:label xml:lang="en">geographic place or region not known (deprecated)</rdfs:label>
        <owl:deprecated rdf:datatype="http://www.w3.org/2001/XMLSchema#boolean">true</owl:deprecated>
    </owl:Class>
    


    <!-- http://purl.obolibrary.org/obo/FOODON_03520199 -->

    <owl:Class rdf:about="http://purl.obolibrary.org/obo/FOODON_03520199">
        <rdfs:subClassOf rdf:resource="http://www.geneontology.org/formats/oboInOwl#ObsoleteClass"/>
        <obo:IAO_0000412>http://langual.org</obo:IAO_0000412>
        <oboInOwl:hasDbXref>LANGUAL:R0199</oboInOwl:hasDbXref>
        <rdfs:comment xml:lang="en">LanguaL curation note: This term is only kept for backward compatibility. DO NOT USE for new indexing.</rdfs:comment>
        <rdfs:label xml:lang="en">czechoslovakia (deprecated)</rdfs:label>
        <owl:deprecated rdf:datatype="http://www.w3.org/2001/XMLSchema#boolean">true</owl:deprecated>
    </owl:Class>
    


    <!-- http://purl.obolibrary.org/obo/FOODON_03530001 -->

    <owl:Class rdf:about="http://purl.obolibrary.org/obo/FOODON_03530001">
        <rdfs:subClassOf rdf:resource="http://www.geneontology.org/formats/oboInOwl#ObsoleteClass"/>
        <obo:IAO_0000412>http://langual.org</obo:IAO_0000412>
        <oboInOwl:hasDbXref>LANGUAL:Z0001</oboInOwl:hasDbXref>
        <rdfs:label xml:lang="en">adjunct characteristics of food not known (deprecated)</rdfs:label>
        <owl:deprecated rdf:datatype="http://www.w3.org/2001/XMLSchema#boolean">true</owl:deprecated>
    </owl:Class>
    


    <!-- http://purl.obolibrary.org/obo/FOODON_03530003 -->

    <owl:Class rdf:about="http://purl.obolibrary.org/obo/FOODON_03530003">
        <rdfs:subClassOf rdf:resource="http://www.geneontology.org/formats/oboInOwl#ObsoleteClass"/>
        <obo:IAO_0000412>http://langual.org</obo:IAO_0000412>
        <oboInOwl:hasDbXref>LANGUAL:Z0003</oboInOwl:hasDbXref>
        <rdfs:comment xml:lang="en">LanguaL curation note: Used only for poultry meat that comes from the back, the neck or for which the color is not known.</rdfs:comment>
        <rdfs:label xml:lang="en">meat color, undesignated or unknown (deprecated)</rdfs:label>
        <owl:deprecated rdf:datatype="http://www.w3.org/2001/XMLSchema#boolean">true</owl:deprecated>
    </owl:Class>
    


    <!-- http://purl.obolibrary.org/obo/FOODON_03530018 -->

    <owl:Class rdf:about="http://purl.obolibrary.org/obo/FOODON_03530018">
        <rdfs:subClassOf rdf:resource="http://www.geneontology.org/formats/oboInOwl#ObsoleteClass"/>
        <obo:IAO_0000412>http://langual.org</obo:IAO_0000412>
        <oboInOwl:hasDbXref>LANGUAL:Z0018</oboInOwl:hasDbXref>
        <rdfs:label xml:lang="en">cut of meat not known (deprecated)</rdfs:label>
        <owl:deprecated rdf:datatype="http://www.w3.org/2001/XMLSchema#boolean">true</owl:deprecated>
    </owl:Class>
    


    <!-- http://purl.obolibrary.org/obo/FOODON_03530019 -->

    <owl:Class rdf:about="http://purl.obolibrary.org/obo/FOODON_03530019">
        <rdfs:subClassOf rdf:resource="http://www.geneontology.org/formats/oboInOwl#ObsoleteClass"/>
        <obo:IAO_0000412>http://langual.org</obo:IAO_0000412>
        <oboInOwl:hasDbXref>LANGUAL:Z0019</oboInOwl:hasDbXref>
        <rdfs:label xml:lang="en">grade of meat not known (deprecated)</rdfs:label>
        <owl:deprecated rdf:datatype="http://www.w3.org/2001/XMLSchema#boolean">true</owl:deprecated>
    </owl:Class>
    


    <!-- http://purl.obolibrary.org/obo/FOODON_03530048 -->

    <owl:Class rdf:about="http://purl.obolibrary.org/obo/FOODON_03530048">
        <rdfs:subClassOf rdf:resource="http://www.geneontology.org/formats/oboInOwl#ObsoleteClass"/>
        <obo:IAO_0000412>http://langual.org</obo:IAO_0000412>
        <oboInOwl:hasDbXref>LANGUAL:Z0048</oboInOwl:hasDbXref>
        <rdfs:label xml:lang="en">cut of meat, other (deprecated)</rdfs:label>
        <owl:deprecated rdf:datatype="http://www.w3.org/2001/XMLSchema#boolean">true</owl:deprecated>
    </owl:Class>
    


    <!-- http://purl.obolibrary.org/obo/FOODON_03530061 -->

    <owl:Class rdf:about="http://purl.obolibrary.org/obo/FOODON_03530061">
        <rdfs:subClassOf rdf:resource="http://www.geneontology.org/formats/oboInOwl#ObsoleteClass"/>
        <obo:IAO_0000412>http://langual.org</obo:IAO_0000412>
        <oboInOwl:hasDbXref>LANGUAL:Z0061</oboInOwl:hasDbXref>
        <rdfs:label xml:lang="en">color of fish flesh not known (deprecated)</rdfs:label>
        <owl:deprecated rdf:datatype="http://www.w3.org/2001/XMLSchema#boolean">true</owl:deprecated>
    </owl:Class>
    


    <!-- http://purl.obolibrary.org/obo/FOODON_03530095 -->

    <owl:Class rdf:about="http://purl.obolibrary.org/obo/FOODON_03530095">
        <rdfs:subClassOf rdf:resource="http://www.geneontology.org/formats/oboInOwl#ObsoleteClass"/>
        <obo:IAO_0000412>http://langual.org</obo:IAO_0000412>
        <oboInOwl:hasDbXref>LANGUAL:Z0095</oboInOwl:hasDbXref>
        <rdfs:label xml:lang="en">sausage casing not known (deprecated)</rdfs:label>
        <owl:deprecated rdf:datatype="http://www.w3.org/2001/XMLSchema#boolean">true</owl:deprecated>
    </owl:Class>
    


    <!-- http://purl.obolibrary.org/obo/FOODON_03530205 -->

    <owl:Class rdf:about="http://purl.obolibrary.org/obo/FOODON_03530205">
        <rdfs:subClassOf rdf:resource="http://www.geneontology.org/formats/oboInOwl#ObsoleteClass"/>
        <obo:IAO_0000412>http://langual.org</obo:IAO_0000412>
        <oboInOwl:hasDbXref>LANGUAL:Z0205</oboInOwl:hasDbXref>
        <rdfs:label xml:lang="en">maturity or ripeness unknown (deprecated)</rdfs:label>
        <owl:deprecated rdf:datatype="http://www.w3.org/2001/XMLSchema#boolean">true</owl:deprecated>
    </owl:Class>
    


    <!-- http://purl.obolibrary.org/obo/FOODON_03530215 -->

    <owl:Class rdf:about="http://purl.obolibrary.org/obo/FOODON_03530215">
        <rdfs:subClassOf rdf:resource="http://www.geneontology.org/formats/oboInOwl#ObsoleteClass"/>
        <obo:IAO_0000412>http://langual.org</obo:IAO_0000412>
        <oboInOwl:hasDbXref>LANGUAL:Z0215</oboInOwl:hasDbXref>
        <rdfs:label xml:lang="en">production environment not known (deprecated)</rdfs:label>
        <owl:deprecated rdf:datatype="http://www.w3.org/2001/XMLSchema#boolean">true</owl:deprecated>
    </owl:Class>
    


    <!-- http://purl.obolibrary.org/obo/FOODON_03530216 -->

    <owl:Class rdf:about="http://purl.obolibrary.org/obo/FOODON_03530216">
        <rdfs:subClassOf rdf:resource="http://www.geneontology.org/formats/oboInOwl#ObsoleteClass"/>
        <obo:IAO_0000412>http://langual.org</obo:IAO_0000412>
        <oboInOwl:hasDbXref>LANGUAL:Z0216</oboInOwl:hasDbXref>
        <rdfs:label xml:lang="en">production environment other (deprecated)</rdfs:label>
        <owl:deprecated rdf:datatype="http://www.w3.org/2001/XMLSchema#boolean">true</owl:deprecated>
    </owl:Class>
    


    <!-- http://purl.obolibrary.org/obo/FOODON_03530262 -->

    <owl:Class rdf:about="http://purl.obolibrary.org/obo/FOODON_03530262">
        <rdfs:subClassOf rdf:resource="http://www.geneontology.org/formats/oboInOwl#ObsoleteClass"/>
        <obo:IAO_0000412>http://langual.org</obo:IAO_0000412>
        <oboInOwl:hasDbXref>LANGUAL:Z0262</oboInOwl:hasDbXref>
        <rdfs:comment xml:lang="en">LanguaL curation note: This term is for CLASSIFICATION ONLY; DO NOT USE term in indexing. Use a more precise narrower term.</rdfs:comment>
        <rdfs:label xml:lang="en">food content range, other (deprecated)</rdfs:label>
        <owl:deprecated rdf:datatype="http://www.w3.org/2001/XMLSchema#boolean">true</owl:deprecated>
    </owl:Class>
    


    <!-- http://www.geneontology.org/formats/oboInOwl#ObsoleteClass -->

    <owl:Class rdf:about="http://www.geneontology.org/formats/oboInOwl#ObsoleteClass"/>
</rdf:RDF>



<!-- Generated by the OWL API (version 4.2.8.20170104-2310) https://github.com/owlcs/owlapi -->

